[this] introducing this, not finished, need exact types

theories/interp.v
@@ -158,12 +158,12 @@ Section proofs.
   Definition interp_nothing : interp Θ :=
     Interp (λ (_: value), False%I).
 
-  Notation ty_interpO := (lang_ty -d> listO (interpO Θ) -n> interpO Θ).
+  Notation ty_interpO := (lang_ty -d> interpO Θ -n> listO (interpO Θ) -n> interpO Θ).
 
-  Lemma ty_interpO_ne : ∀ (rec: ty_interpO) ty, NonExpansive (rec ty).
+  Lemma ty_interpO_ne : ∀ (rec: ty_interpO) ty Σthis, NonExpansive (rec ty Σthis).
   Proof.
     move => rec ty.
-    apply _.
+    by apply _.
   Qed.
 
   Definition interp_variance (v: variance) (i0 i1: interp Θ) : iProp Θ :=
@@ -276,9 +276,10 @@ Section proofs.
    * for example about `seal`.
    *)
   Definition interp_tag_def
-    (rec : ty_interpO)
-    (Σ : list (interp Θ))
+    (rec: ty_interpO)
     (C: tag)
+    (Σthis: interp Θ)
+    (Σ : list (interp Θ))
     : interp Θ :=
     Interp (
       λ (w : value), (∃ ℓ t cdef tdef σ (Σt: list (interp Θ))
@@ -293,214 +294,91 @@ Section proofs.
        dom fields = dom ifields⌝ ∗
 
       □ ▷ (∀ i (ϕi: interp Θ),  ⌜Σt !! i = Some ϕi⌝ →
-           ∀ v,  ϕi v -∗ rec MixedT [] v) ∗
-
+           ∀ v,  ϕi v -∗ rec MixedT Σthis [] v) ∗
+      (* Constraints can't mention `this` *)
       □ ▷ (∀ i c, ⌜tdef.(constraints) !! i = Some c⌝ →
-           ∀ v, rec c.1 Σt v -∗ rec c.2 Σt v) ∗
-
-      □ ▷ (∀ k v (i0 i1: interp Θ),
+           ∀ v, rec c.1 Σthis Σt v -∗ rec c.2 Σthis Σt v) ∗
+      (* Extend clauses can't mention `this` *)
+      □ ▷ (∀ k v i0 i1,
          ⌜cdef.(generics) !! k = Some v⌝ →
-         ((λ ty, rec ty Σt) <$> σ) !! k ≡ Some i0 →
+         ((λ ty, rec ty Σthis Σt) <$> σ) !! k ≡ Some i0 →
          Σ !! k ≡ Some i1 →
          interp_variance v i0 i1) ∗
 
       ▷ (∀ f vis ty orig, ⌜has_field f t vis ty orig⌝ -∗
-          (ifields !! f ≡ Some (interp_car (rec ty Σt)))) ∗
+          (ifields !! f ≡ Some (interp_car (rec ty Σthis Σt)))) ∗
 
       (ℓ ↦ (t, ifields)))%I
     ).
 
-   Local Definition interp_tag_aux
-     (rec : ty_interpO) (Σ : list (interp Θ)) (C: tag)
-     : seal (@interp_tag_def rec Σ C).
+   Local Definition interp_tag_aux (rec : ty_interpO) C Σthis Σ
+     : seal (@interp_tag_def rec C Σthis Σ).
    Proof. by eexists. Qed.
 
-   Definition interp_tag (rec: ty_interpO) (Σ: list (interp Θ)) (C: tag) :=
-     (interp_tag_aux rec Σ C).(unseal).
+   Definition interp_tag (rec : ty_interpO) C Σthis Σ :=
+     (interp_tag_aux rec C Σthis Σ).(unseal).
 
-   Definition interp_tag_unseal
-     (rec : ty_interpO) (Σ : list (interp Θ)) (C: tag)
-     : interp_tag rec Σ C = interp_tag_def rec Σ C :=
-     (interp_tag_aux rec Σ C).(seal_eq).
+   Definition interp_tag_unseal (rec : ty_interpO) C Σthis Σ:
+     interp_tag rec C Σthis Σ = interp_tag_def rec C Σthis Σ :=
+     (interp_tag_aux rec C Σthis Σ).(seal_eq).
 
-  Definition interp_exact_tag_def
-    (rec : ty_interpO)
-    (Σ : list (interp Θ))
-    (C: tag)
-    : interp Θ :=
-    Interp (
-      λ (w : value), (∃ ℓ cdef (Σc: list (interp Θ))
-       (fields: stringmap ((visibility * lang_ty) * tag))
-       (ifields: gmapO string (sem_typeO Θ)),
-      ⌜w = LocV ℓ ∧
-       pdefs !! C = Some cdef ∧
-       length Σc = length cdef.(generics) ∧
-       has_fields C fields ∧
-       dom fields = dom ifields⌝ ∗
+   Local Instance interp_tag_ne C Σthis (rec: ty_interpO):
+     NonExpansive (λ Σ, interp_tag rec C Σthis Σ).
+   Proof.
+     move => n x y h.
+     rewrite !interp_tag_unseal /interp_tag_def => v.
+     rewrite /interp_fun !interp_car_simpl /interp_variance.
+     by repeat f_equiv.
+   Qed.
 
-      □ ▷ (∀ i (ϕi: interp Θ),  ⌜Σc !! i = Some ϕi⌝ →
-           ∀ v,  ϕi v -∗ rec MixedT [] v) ∗
+   Local Instance interp_tag_this_ne C Σ (rec: ty_interpO):
+     NonExpansive (λ Σthis, interp_tag rec C Σthis Σ).
+   Proof.
+     move => n x y h.
+     rewrite !interp_tag_unseal /interp_tag_def => v.
+     rewrite /interp_fun !interp_car_simpl /interp_variance.
+     do 18 f_equiv.
+     { do 12 f_equiv.
+       by rewrite h.
+     }
+     f_equiv.
+     { by repeat f_equiv. }
+     f_equiv.
+     { do 14 f_equiv.
+       apply list_fmap_ext_ne => ty.
+       f_equiv.
+       by rewrite h.
+     }
+     by repeat f_equiv.
+   Qed.
 
-      □ ▷ (∀ i c, ⌜cdef.(constraints) !! i = Some c⌝ →
-           ∀ v, rec c.1 Σc v -∗ rec c.2 Σc v) ∗
+   Local Instance interp_tag_this_contractive C Σ (rec: ty_interpO):
+     Contractive (λ Σthis, interp_tag rec C Σthis Σ).
+   Proof.
+     move => n x y h.
+     rewrite !interp_tag_unseal /interp_tag_def => v.
+     rewrite /interp_fun !interp_car_simpl /interp_variance.
+     do 18 f_equiv.
+     { f_equiv; f_contractive.
+       do 10 f_equiv.
+       by rewrite h.
+     }
+     f_equiv.
+     { f_equiv; f_contractive; by repeat f_equiv. }
+     f_equiv.
+     { f_equiv; f_contractive.
+       do 12 f_equiv.
+       apply list_fmap_ext_ne => ty.
+       f_equiv.
+       by rewrite h.
+     }
+     f_equiv.
+     f_contractive.
+     by repeat f_equiv.
+   Qed.
 
-      □ ▷ (∀ k v (i0 i1: interp Θ),
-         ⌜cdef.(generics) !! k = Some v⌝ →
-         Σc!! k ≡ Some i0 →
-         Σ !! k ≡ Some i1 →
-         interp_variance v i0 i1) ∗
-
-      ▷ (∀ f vis ty orig, ⌜has_field f C vis ty orig⌝ -∗
-          (ifields !! f ≡ Some (interp_car (rec ty Σc)))) ∗
-
-      (ℓ ↦ (C, ifields)))%I
-    ).
-
-   Local Definition interp_exact_tag_aux
-     (rec : ty_interpO) (Σ : list (interp Θ)) (C: tag)
-     : seal (@interp_exact_tag_def rec Σ C).
-   Proof. by eexists. Qed.
-
-   Definition interp_exact_tag (rec: ty_interpO) (Σ: list (interp Θ)) (C: tag) :=
-     (interp_exact_tag_aux rec Σ C).(unseal).
-
-   Definition interp_exact_tag_unseal
-     (rec : ty_interpO) (Σ : list (interp Θ)) (C: tag)
-     : interp_exact_tag rec Σ C = interp_exact_tag_def rec Σ C :=
-     (interp_exact_tag_aux rec Σ C).(seal_eq).
-
-  Definition interp_nonnull (rec : ty_interpO) : interp Θ :=
-    Interp (
-      λ (v : value),
-      ((interp_int v) ∨
-      (interp_bool v) ∨
-      (∃ t Σ tdef, ⌜pdefs !! t = Some tdef ∧
-        length Σ = length tdef.(generics)⌝ ∗
-        interp_tag rec Σ t v))%I
-    ).
-
-  Definition interp_mixed (rec: ty_interpO) : interp Θ :=
-    Interp (λ (v: value), (interp_nonnull rec v ∨ interp_null v)%I).
-
-  Definition interp_generic (Σ : list (interp Θ)) (tv: nat) : interp Θ :=
-    default interp_nothing (Σ !! tv).
-
-  Definition interp_sdt (rec: ty_interpO) : interp Θ :=
-    Interp (λ (v: value),
-      (∃ A Σa adef, ⌜pdefs !! A = Some adef ∧
-        length Σa = length adef.(generics)⌝ ∗
-      (* Σa |= Δsdt A *)
-      □ ▷ (∀ i c, ⌜Δsdt A !! i = Some c⌝ →
-        ∀ w, rec c.1 Σa w -∗ rec c.2 Σa w) ∗
-      (* Σa included in [| mixed |] *)
-      □ ▷ (∀ i (ϕi: interp Θ),  ⌜Σa !! i = Some ϕi⌝ →
-        ∀ v,  ϕi v -∗ rec MixedT [] v) ∗
-      (* Σa |= Δa *)
-      □ ▷ (∀ i c, ⌜adef.(constraints) !! i = Some c⌝ →
-           ∀ v, rec c.1 Σa v -∗ rec c.2 Σa v) ∗
-      interp_tag rec Σa A v))%I.
-
-  Definition interp_support_dynamic (rec: ty_interpO) : interp Θ :=
-    Interp (λ (v: value),
-      interp_int v ∨
-      interp_bool v ∨
-      interp_null v ∨
-      interp_sdt rec v)%I.
-
-  Definition interp_dynamic (rec: ty_interpO) : interp Θ :=
-    interp_support_dynamic rec.
-
-  (* we use a blend of Coq/Iris recursion, the
-     Coq recursion lets us handle simple structural
-     cases, and we use Iris' recursion to deal with
-     the more complicated case of class types.
-  *)
-  Section interp_type_pre_rec.
-    Variable (rec: ty_interpO).
-
-    Fixpoint go (Σ: listO (interpO Θ)) (typ: lang_ty) : interp Θ :=
-      match typ with
-      | IntT => interp_int
-      | BoolT => interp_bool
-      | NothingT => interp_nothing
-      | MixedT => interp_mixed rec
-      | ClassT true A σA =>
-          let Σ := (go Σ) <$> σA in
-          interp_exact_tag rec Σ A
-      | ClassT false A σA =>
-          let Σ := (go Σ) <$> σA in
-          interp_tag rec Σ A
-      | NullT => interp_null
-      | NonNullT => interp_nonnull rec
-      | UnionT A B => interp_union (go Σ A) (go Σ B)
-      | InterT A B => interp_inter (go Σ A) (go Σ B)
-      | GenT n => interp_generic Σ n
-      | DynamicT => interp_dynamic rec
-      | SupportDynT => interp_support_dynamic rec
-      end.
-  End interp_type_pre_rec.
-
- Local Instance interp_tag_ne C (rec: ty_interpO) :
-    NonExpansive (λ Σ, interp_tag rec Σ C).
-  Proof.
-    move => n x y h.
-    rewrite !interp_tag_unseal /interp_tag_def => v.
-    rewrite /interp_fun !interp_car_simpl /interp_variance.
-    by repeat f_equiv.
-  Qed.
-
- Local Instance interp_exact_tag_ne C (rec: ty_interpO) :
-    NonExpansive (λ Σ, interp_exact_tag rec Σ C).
-  Proof.
-    move => n x y h.
-    rewrite !interp_exact_tag_unseal /interp_exact_tag_def => v.
-    rewrite /interp_fun !interp_car_simpl.
-    by repeat f_equiv.
-  Qed.
-
-  Local Instance go_ne (rec: ty_interpO) (ty: lang_ty) :
-    NonExpansive (λ Σ, go rec Σ ty).
-  Proof.
-    elim: ty => //=.
-    - move => exact_ t σ hi n x y h.
-      assert (heq : go rec x <$> σ ≡{n}≡ go rec y <$> σ).
-      { rewrite Forall_lookup in hi.
-        apply list_dist_lookup => k.
-        rewrite !list_lookup_fmap.
-        destruct (σ !! k) as [ ty | ] eqn:hty => //=.
-        f_equiv.
-        apply hi with (n := n) in hty.
-        by apply hty.
-      }
-      destruct exact_.
-      + by apply interp_exact_tag_ne.
-      + by apply interp_tag_ne.
-    - move => A B hA hB n x y h v /=.
-      f_equiv.
-      + revert v; by apply hA.
-      + revert v; by apply hB.
-    - move => A B hA hB n x y h v /=.
-      f_equiv.
-      + revert v; by apply hA.
-      + revert v; by apply hB.
-    - move => k n x y h v /=.
-      assert (hl: length x = length y) by now apply Forall2_length in h.
-      elim : x y k h hl => [ | hd tl hi]; case => [ | hd' tl'] i h /= hl => //.
-      apply Forall2_cons in h as [hhd htl].
-      case: i hi => [ | i ] hi //=.
-      apply: hi; first done.
-      by lia.
-  Qed.
-
-  Definition interp_type_pre (rec : ty_interpO) : ty_interpO :=
-    λ (typ : lang_ty), λne (Σ: listO (interpO Θ)), go rec Σ typ.
-
-  Global Instance interp_type_pre_persistent (rec: ty_interpO) :
-    ∀ t σi v, Persistent (interp_type_pre rec t σi v).
-  Proof. by move => ???; apply _. Qed.
-
-  Global Instance interp_tag_contractive Σ C:
-    Contractive (λ rec, interp_tag rec Σ C).
+  Global Instance interp_tag_contractive C Σthis Σ:
+    Contractive (λ rec, interp_tag rec C Σthis Σ).
   Proof.
     move => n x y h.
     rewrite !interp_tag_unseal /interp_tag_def => v.
@@ -525,18 +403,349 @@ Section proofs.
     by repeat f_equiv.
   Qed.
 
+  Definition interp_class (rec: ty_interpO) (t: tag) (Σ: list (interp Θ)) : interp Θ :=
+    Interp (λ (w: value),
+     (∃ (Σthis : interp Θ),
+       (* ""this included in t<this>"" *)
+      □ ▷ (∀ v, Σthis v -∗ interp_tag rec t Σthis Σ v) ∗
+      (* Σthis included in [| mixed |] *)
+      □ ▷ (∀ v,  Σthis v -∗ rec MixedT Σthis [] v) ∗
+       interp_tag rec t Σthis Σ w))%I.
+
+  Definition interp_exact_tag_def
+    (rec : ty_interpO)
+    (C: tag)
+    (Σthis : interp Θ)
+    (Σ : list (interp Θ))
+    : interp Θ :=
+    Interp (
+      λ (w : value), (∃ ℓ cdef (Σc: list (interp Θ))
+       (fields: stringmap ((visibility * lang_ty) * tag))
+       (ifields: gmapO string (sem_typeO Θ)),
+      ⌜w = LocV ℓ ∧
+       pdefs !! C = Some cdef ∧
+       length Σc = length cdef.(generics) ∧
+       has_fields C fields ∧
+       dom fields = dom ifields⌝ ∗
+
+      □ ▷ (∀ i (ϕi: interp Θ),  ⌜Σc !! i = Some ϕi⌝ →
+           ∀ v,  ϕi v -∗ rec MixedT Σthis [] v) ∗
+
+      □ ▷ (∀ i c, ⌜cdef.(constraints) !! i = Some c⌝ →
+           ∀ v, rec c.1 Σthis Σc v -∗ rec c.2 Σthis Σc v) ∗
+
+      □ ▷ (∀ k v (i0 i1: interp Θ),
+         ⌜cdef.(generics) !! k = Some v⌝ →
+         Σc!! k ≡ Some i0 →
+         Σ !! k ≡ Some i1 →
+         interp_variance v i0 i1) ∗
+
+      ▷ (∀ f vis ty orig, ⌜has_field f C vis ty orig⌝ -∗
+          (ifields !! f ≡ Some (interp_car (rec ty Σthis Σc)))) ∗
+
+      (ℓ ↦ (C, ifields)))%I
+    ).
+
+   Local Definition interp_exact_tag_aux
+     (rec : ty_interpO) C (Σthis : interp Θ) (Σ : list (interp Θ))
+     : seal (@interp_exact_tag_def rec C Σthis Σ).
+   Proof. by eexists. Qed.
+
+   Definition interp_exact_tag (rec: ty_interpO) C (Σthis: interp Θ)
+     (Σ: list (interp Θ)) :=
+     (interp_exact_tag_aux rec C Σthis Σ).(unseal).
+
+   Definition interp_exact_tag_unseal
+     (rec : ty_interpO) C (Σthis: interp Θ) (Σ : list (interp Θ))
+     : interp_exact_tag rec C Σthis Σ = interp_exact_tag_def rec C Σthis Σ :=
+     (interp_exact_tag_aux rec C Σthis Σ).(seal_eq).
+
+ Local Instance interp_exact_tag_ne C Σthis (rec: ty_interpO) :
+    NonExpansive (λ Σ, interp_exact_tag rec C Σthis Σ).
+  Proof.
+    move => n x y h.
+    rewrite !interp_exact_tag_unseal /interp_exact_tag_def => v.
+    rewrite /interp_fun !interp_car_simpl.
+    by repeat f_equiv.
+  Qed.
+
+   Local Instance interp_exact_tag_this_ne C Σ (rec: ty_interpO):
+     NonExpansive (λ Σthis, interp_exact_tag rec C Σthis Σ).
+   Proof.
+     move => n x y h.
+     rewrite !interp_exact_tag_unseal /interp_exact_tag_def => v.
+     rewrite /interp_fun !interp_car_simpl /interp_variance.
+     do 12 f_equiv.
+     { do 12 f_equiv.
+       by rewrite h.
+     }
+     f_equiv.
+     { by repeat f_equiv. }
+     by repeat f_equiv.
+   Qed.
+
+   Local Instance interp_exact_tag_this_contractive C Σ (rec: ty_interpO):
+     Contractive (λ Σthis, interp_exact_tag rec C Σthis Σ).
+   Proof.
+     move => n x y h.
+     rewrite !interp_exact_tag_unseal /interp_exact_tag_def => v.
+     rewrite /interp_fun !interp_car_simpl /interp_variance.
+     do 12 f_equiv.
+     { f_equiv; f_contractive.
+       do 10 f_equiv.
+       by rewrite h.
+     }
+     f_equiv.
+     { f_equiv; f_contractive; by repeat f_equiv. }
+     f_equiv.
+     f_equiv.
+     f_contractive.
+     by repeat f_equiv.
+   Qed.
+
+  Global Instance interp_exact_tag_contractive C Σthis Σ:
+    Contractive (λ rec, interp_exact_tag rec C Σthis Σ).
+  Proof.
+    move => n x y h.
+    rewrite !interp_exact_tag_unseal /interp_exact_tag_def => v.
+    rewrite /interp_fun !interp_car_simpl /interp_variance.
+    do 12 f_equiv.
+    { f_equiv; f_contractive.
+      by repeat f_equiv.
+    }
+    f_equiv.
+    { f_equiv; f_contractive.
+      by repeat f_equiv.
+    }
+    f_equiv.
+    f_equiv; f_contractive.
+    by repeat f_equiv.
+  Qed.
+
+  Definition interp_exact_class (rec: ty_interpO) (t: tag) (Σ: list (interp Θ)) : interp Θ :=
+    Interp (λ (w: value),
+     (∃ (Σthis : interp Θ),
+       (* ""this included in t<this>"" *)
+      □ ▷ (∀ v, Σthis v -∗ interp_exact_tag rec t Σthis Σ v) ∗
+      (* Σthis included in [| mixed |] *)
+      □ ▷ (∀ v,  Σthis v -∗ rec MixedT Σthis [] v) ∗
+       interp_exact_tag rec t Σthis Σ w))%I.
+
+  Definition interp_nonnull (rec : ty_interpO) : interp Θ :=
+    Interp (
+      λ (v : value),
+      ((interp_int v) ∨
+      (interp_bool v) ∨
+      (∃ t (Σ: list (interp Θ)) tdef, ⌜pdefs !! t = Some tdef ∧
+        length Σ = length tdef.(generics)⌝ ∗
+        interp_class rec t Σ v))%I
+    ).
+
+  Definition interp_mixed (rec: ty_interpO) : interp Θ :=
+    Interp (λ (v: value), (interp_nonnull rec v ∨ interp_null v)%I).
+
+  Definition interp_generic (Σ: list (interp Θ)) (tv: nat) : interp Θ :=
+    default interp_nothing (Σ !! tv).
+
+  Definition interp_sdt (rec: ty_interpO) : interp Θ :=
+    Interp (λ (v: value),
+      (∃ A Σthisa (Σa: list (interp Θ)) adef, ⌜pdefs !! A = Some adef ∧
+        length Σa = length adef.(generics)⌝ ∗
+      (* Σa |= Δsdt A *)
+      □ ▷ (∀ i c, ⌜Δsdt A !! i = Some c⌝ →
+        ∀ w, rec c.1 Σthisa Σa w -∗ rec c.2 Σthisa Σa w) ∗
+      (* Σa included in [| mixed |] *)
+      □ ▷ (∀ i (ϕi: interp Θ),  ⌜Σa !! i = Some ϕi⌝ →
+        ∀ v,  ϕi v -∗ rec MixedT Σthisa [] v) ∗
+      (* Σa |= Δa *)
+      □ ▷ (∀ i c, ⌜adef.(constraints) !! i = Some c⌝ →
+           ∀ v, rec c.1 Σthisa Σa v -∗ rec c.2 Σthisa Σa v) ∗
+      (* `this` conditions *)
+      □ ▷ (∀ v, Σthisa v -∗ interp_tag rec A Σthisa Σa v) ∗
+      □ ▷ (∀ v, Σthisa v -∗ rec MixedT Σthisa [] v) ∗
+      interp_tag rec A Σthisa Σa v))%I.
+
+  Definition interp_support_dynamic (rec: ty_interpO) : interp Θ :=
+    Interp (λ (v: value),
+      interp_int v ∨
+      interp_bool v ∨
+      interp_null v ∨
+      interp_sdt rec v)%I.
+
+  Definition interp_dynamic (rec: ty_interpO) : interp Θ :=
+    interp_support_dynamic rec.
+
+  (* we use a blend of Coq/Iris recursion, the
+     Coq recursion lets us handle simple structural
+     cases, and we use Iris' recursion to deal with
+     the more complicated case of class types.
+  *)
+  Section interp_type_pre_rec.
+    Variable (rec: ty_interpO).
+    Variable (Σthis : interp Θ).
+
+    Fixpoint go (Σ: list (interp Θ)) (typ: lang_ty) : interp Θ :=
+      match typ with
+      | IntT => interp_int
+      | BoolT => interp_bool
+      | NothingT => interp_nothing
+      | MixedT => interp_mixed rec
+      | ClassT true A σA =>
+          let Σ := (go Σ) <$> σA in
+          interp_exact_class rec A Σ
+      | ClassT false A σA =>
+          let Σ := (go Σ) <$> σA in
+          interp_class rec A Σ
+      | NullT => interp_null
+      | NonNullT => interp_nonnull rec
+      | UnionT A B => interp_union (go Σ A) (go Σ B)
+      | InterT A B => interp_inter (go Σ A) (go Σ B)
+      | GenT n => interp_generic Σ n
+      | DynamicT => interp_dynamic rec
+      | SupportDynT => interp_support_dynamic rec
+      | ThisT => Σthis
+      end.
+  End interp_type_pre_rec.
+
+  Local Instance interp_class_ne (rec: ty_interpO) t :
+    NonExpansive (λ Σ, interp_class rec t Σ).
+  Proof.
+    rewrite /interp_class => n x y h v /=.
+    do 3 f_equiv.
+    { do 5 f_equiv.
+      by apply interp_tag_ne.
+    }
+    f_equiv.
+    by apply interp_tag_ne.
+  Qed.
+
+  Local Instance interp_exact_class_ne (rec: ty_interpO) t :
+    NonExpansive (λ Σ, interp_exact_class rec t Σ).
+  Proof.
+    rewrite /interp_exact_class => n x y h v /=.
+    do 3 f_equiv.
+    { do 5 f_equiv.
+      by apply interp_exact_tag_ne.
+    }
+    f_equiv.
+    by apply interp_exact_tag_ne.
+  Qed.
+
+
+  Local Instance go_ne (rec: ty_interpO) Σthis (ty: lang_ty) :
+    NonExpansive (λ Σ, go rec Σthis Σ ty).
+  Proof.
+    elim: ty => //=.
+    - move => exact_ t σ hi n x y h.
+      assert (heq : go rec Σthis x <$> σ ≡{n}≡ go rec Σthis y <$> σ).
+      { rewrite Forall_lookup in hi.
+        apply list_dist_lookup => k.
+        rewrite !list_lookup_fmap.
+        destruct (σ !! k) as [ ty | ] eqn:hty => //=.
+        f_equiv.
+        apply hi with (n := n) in hty.
+        by apply hty.
+      }
+      destruct exact_.
+      + by apply interp_exact_class_ne.
+      + by apply interp_class_ne.
+    - move => A B hA hB n x y h v /=.
+      f_equiv.
+      + revert v; by apply hA.
+      + revert v; by apply hB.
+    - move => A B hA hB n x y h v /=.
+      f_equiv.
+      + revert v; by apply hA.
+      + revert v; by apply hB.
+    - move => k n x y h v /=.
+      assert (hl: length x = length y) by now apply Forall2_length in h.
+      elim : x y k h hl => [ | hd tl hi]; case => [ | hd' tl'] i h /= hl => //.
+      apply Forall2_cons in h as [hhd htl].
+      case: i hi => [ | i ] hi //=.
+      apply: hi; first done.
+      by lia.
+  Qed.
+
+  Local Instance go_this_ne (rec: ty_interpO) (ty: lang_ty) :
+    NonExpansive (λ Σthis, λne Σ, go rec Σthis Σ ty).
+  Proof.
+    elim : ty => //=.
+    - move => exact_ t σ hi n x y h Σ v /=.
+      assert (heq: go rec x Σ <$> σ ≡{n}≡ go rec y Σ <$> σ).
+      { rewrite Forall_lookup in hi.
+        apply list_dist_lookup => k.
+        rewrite !list_lookup_fmap.
+        destruct (σ !! k) as [ty | ] eqn:hty => //=.
+        f_equiv.
+        apply hi with (n := n) in hty.
+        by apply hty.
+      }
+      destruct exact_.
+      + by apply interp_exact_class_ne.
+      + by apply interp_class_ne.
+    - move => A B hA hB n x y h Σ v /=.
+      f_equiv.
+      + revert v; by apply hA.
+      + revert v; by apply hB.
+    - move => A B hA hB n x y h Σ v /=.
+      f_equiv.
+      + revert v; by apply hA.
+      + revert v; by apply hB.
+    - move => n x y h Σ v /=.
+      by rewrite h.
+  Qed.
+
+  Definition interp_type_pre (rec : ty_interpO) : ty_interpO :=
+    λ (typ : lang_ty), λne (Σthis: interp Θ), λne Σ, go rec Σthis Σ typ.
+
+  Global Instance interp_type_pre_persistent (rec: ty_interpO) :
+    ∀ t Σthis Σ v, Persistent (interp_type_pre rec t Σthis Σ v).
+  Proof. by move => ???; apply _. Qed.
+
+  Global Instance interp_class_contractive t Σ :
+    Contractive (λ rec, interp_class rec t Σ).
+  Proof.
+    rewrite /interp_class => n i1 i2 hdist v.
+    rewrite /interp_fun !interp_car_simpl.
+    do 3 f_equiv.
+    { do 5 f_equiv.
+      by apply interp_tag_contractive.
+    }
+    f_equiv.
+    { f_equiv; f_contractive.
+      by repeat f_equiv.
+    }
+    by apply interp_tag_contractive.
+  Qed.
+
+  Global Instance interp_exact_class_contractive t Σ :
+    Contractive (λ rec, interp_exact_class rec t Σ).
+  Proof.
+    rewrite /interp_exact_class => n i1 i2 hdist v.
+    rewrite /interp_fun !interp_car_simpl.
+    do 3 f_equiv.
+    { do 5 f_equiv.
+      by apply interp_exact_tag_contractive.
+    }
+    f_equiv.
+    { f_equiv; f_contractive.
+      by repeat f_equiv.
+    }
+    by apply interp_exact_tag_contractive.
+  Qed.
+
   Global Instance interp_nonnull_contractive: Contractive interp_nonnull.
   Proof.
     rewrite /interp_nonnull => n i1 i2 hdist v.
     rewrite /interp_fun !interp_car_simpl.
-    do 9 f_equiv.
-    by apply interp_tag_contractive.
+    do 10 f_equiv.
+    by apply interp_class_contractive.
   Qed.
 
   Local Instance interp_type_pre_contractive : Contractive interp_type_pre.
   Proof.
-    rewrite /interp_type_pre => n rec1 rec2 hdist ty Σ /=.
-    induction ty as [ | | | | exact_ C σ hi | | | A B hA hB | A B hA hB | i | | ] => /=.
+    rewrite /interp_type_pre => n rec1 rec2 hdist ty Σthis Σ /=.
+    induction ty as [ | | | | exact_ C σ hi | | | A B hA hB | A B hA hB | i | | | ] => /=.
     - done.
     - done.
     - done.
@@ -545,88 +754,152 @@ Section proofs.
       f_equiv.
       revert v; by apply interp_nonnull_contractive.
     - destruct exact_.
-      + rewrite !interp_exact_tag_unseal /interp_exact_tag_def => v.
-        rewrite /interp_fun !interp_car_simpl.
-        rewrite Forall_forall in hi.
-        do 12 f_equiv.
-        { f_equiv; f_contractive.
-          by repeat f_equiv.
-        }
-        f_equiv.
-        { f_equiv; f_contractive.
-          by repeat f_equiv.
-        }
-        f_equiv.
-        { f_equiv; f_contractive.
-          do 13 f_equiv.
-          apply Forall2_fmap, Forall_Forall2_diag, Forall_forall => ? hin.
-          apply dist_S.
-          by apply hi.
-        }
-        f_equiv.
-        f_contractive.
-        do 13 f_equiv; first by repeat f_equiv.
-      + rewrite !interp_tag_unseal /interp_tag_def => v.
-        rewrite /interp_fun !interp_car_simpl /interp_variance.
-        rewrite Forall_forall in hi.
-        do 18 f_equiv.
-        { f_equiv; f_contractive.
-          by repeat f_equiv.
-        }
-        f_equiv.
-        { f_equiv; f_contractive.
-          by repeat f_equiv.
-        }
-        f_equiv.
-        { f_equiv; f_contractive.
-          do 10 f_equiv.
-          * do 2 f_equiv.
-            apply Forall2_fmap, Forall_Forall2_diag, Forall_forall => ? hin.
-            by apply hdist.
-          * do 3 f_equiv.
+      + rewrite /interp_exact_class => v /=.
+        assert (htag: ∀ t w,
+          interp_exact_tag rec1 C t (go rec1 Σthis Σ <$> σ) w ≡{n}≡
+          interp_exact_tag rec2 C t (go rec2 Σthis Σ <$> σ) w).
+        { move => t w.
+          rewrite !interp_exact_tag_unseal /interp_exact_tag_def.
+          rewrite /interp_fun !interp_car_simpl /interp_variance.
+          rewrite Forall_forall in hi.
+          do 12 f_equiv.
+          { f_equiv; f_contractive.
+            by repeat f_equiv.
+          }
+          f_equiv.
+          { f_equiv; f_contractive.
+            by repeat f_equiv.
+          }
+          f_equiv.
+          { f_equiv; f_contractive.
+            do 13 f_equiv.
             apply Forall2_fmap, Forall_Forall2_diag, Forall_forall => ? hin.
             apply dist_S.
             by apply hi.
+          }
+          f_equiv.
+          f_contractive.
+          do 11 f_equiv.
+          by apply hdist.
+        }
+        do 3 f_equiv.
+        { f_equiv; f_contractive.
+          do 3 f_equiv.
+          apply dist_S.
+          by apply htag.
         }
         f_equiv.
-        f_contractive.
-        do 11 f_equiv.
-        by apply hdist.
+        { f_equiv; f_contractive.
+          by repeat f_equiv.
+        }
+        by apply htag.
+      + rewrite /interp_class => v /=.
+        assert (htag: ∀ t w,
+          interp_tag rec1 C t (go rec1 Σthis Σ <$> σ) w ≡{n}≡
+          interp_tag rec2 C t (go rec2 Σthis Σ <$> σ) w).
+        { move => t w.
+          rewrite !interp_tag_unseal /interp_tag_def.
+          rewrite /interp_fun !interp_car_simpl /interp_variance.
+          rewrite Forall_forall in hi.
+          do 18 f_equiv.
+          { f_equiv; f_contractive.
+            by repeat f_equiv.
+          }
+          f_equiv.
+          { f_equiv; f_contractive.
+            by repeat f_equiv.
+          }
+          f_equiv.
+          { f_equiv; f_contractive.
+            do 10 f_equiv.
+            * do 2 f_equiv.
+              apply Forall2_fmap, Forall_Forall2_diag, Forall_forall => ? hin.
+              by apply hdist.
+            * do 3 f_equiv.
+              apply Forall2_fmap, Forall_Forall2_diag, Forall_forall => ? hin.
+              apply dist_S.
+              by apply hi.
+          }
+          f_equiv.
+          f_contractive.
+          do 11 f_equiv.
+          by apply hdist.
+        }
+        do 3 f_equiv.
+        { f_equiv; f_contractive.
+          do 3 f_equiv.
+          apply dist_S.
+          by apply htag.
+        }
+        f_equiv.
+        { f_equiv; f_contractive.
+          by repeat f_equiv.
+        }
+        by apply htag.
     - done.
     - by apply interp_nonnull_contractive.
     - by solve_proper_core ltac:(fun _ => first [done | f_contractive | f_equiv]).
     - by solve_proper_core ltac:(fun _ => first [done | f_contractive | f_equiv]).
     - done.
     - rewrite /interp_dynamic /interp_support_dynamic /interp_sdt => v /=.
-      do 11 f_equiv.
+      do 13 f_equiv.
       { f_equiv; f_contractive; by repeat f_equiv. }
       f_equiv.
       { f_equiv; f_contractive; by repeat f_equiv. }
-      f_equiv; last by apply interp_tag_contractive.
+      f_equiv.
       { f_equiv; f_contractive; by repeat f_equiv. }
+      f_equiv.
+      { f_equiv; f_contractive.
+        do 3 f_equiv.
+        apply dist_S.
+        by apply interp_tag_contractive.
+      }
+      f_equiv.
+      { f_equiv; f_contractive.
+        by repeat f_equiv.
+      }
+      by apply interp_tag_contractive.
     - rewrite /interp_dynamic /interp_support_dynamic /interp_sdt => v /=.
-      do 11 f_equiv.
+      do 13 f_equiv.
       { f_equiv; f_contractive; by repeat f_equiv. }
       f_equiv.
       { f_equiv; f_contractive; by repeat f_equiv. }
-      f_equiv; last by apply interp_tag_contractive.
+      f_equiv.
       { f_equiv; f_contractive; by repeat f_equiv. }
+      f_equiv.
+      { f_equiv; f_contractive.
+        do 3 f_equiv.
+        apply dist_S.
+        by apply interp_tag_contractive.
+      }
+      f_equiv.
+      { f_equiv; f_contractive.
+        by repeat f_equiv.
+      }
+      by apply interp_tag_contractive.
+    - done.
   Qed.
+
+  Implicit Types Σ : list (interp Θ).
+  Implicit Types Σthis : interp Θ.
 
   (* the interpretation of types can now be
      defined as a fixpoint (because class types
      can be (mutually) recursive) *)
   Definition interp_type := fixpoint interp_type_pre.
 
-  Definition interp_env_as_mixed (Σ: list (interp Θ)) :=
-    (∀ i (ϕi: interp Θ),  ⌜Σ !! i = Some ϕi⌝ → ∀ v,  ϕi v -∗ interp_mixed interp_type v)%I.
+  (* TODO: use interp_inclusion a bit more, maybe introduce a notation *)
+  Definition interp_inclusion (ϕ0 ϕ1: interp Θ) := (∀ v, ϕ0 v -∗ ϕ1 v)%I.
+  Definition interp_as_mixed ϕ := interp_inclusion ϕ (interp_mixed interp_type).
+  Definition interp_env_as_mixed Σ :=
+    (∀ i (ϕi: interp Θ),  ⌜Σ !! i = Some ϕi⌝ → interp_as_mixed ϕi)%I.
 
-  Definition Σinterp (Σ: list (interp Θ)) (Δ : list constraint) :=
+  Definition Σinterp Σthis Σ (Δ : list constraint) :=
     (∀ i c, ⌜Δ !! i = Some c⌝ →
-    ∀ v, interp_type c.1 Σ v -∗ interp_type c.2 Σ v)%I.
+    ∀ v, interp_type c.1 Σthis Σ v -∗ interp_type c.2 Σthis Σ v)%I.
 
-  Lemma Σinterp_app Σ Δ0 Δ1:
-    Σinterp Σ Δ0 -∗ Σinterp Σ Δ1 -∗ Σinterp Σ (Δ0 ++ Δ1).
+  Lemma Σinterp_app Σthis Σ Δ0 Δ1:
+    Σinterp Σthis Σ Δ0 -∗ Σinterp Σthis Σ Δ1 -∗ Σinterp Σthis Σ (Δ0 ++ Δ1).
   Proof.
     iIntros "h0 h1".
     iIntros (i c hc v) "#h".
@@ -638,52 +911,64 @@ Section proofs.
       by iApply "h1".
   Qed.
 
-  Definition interp_list (Σ: list (interp Θ)) (σ: list lang_ty) :=
-    (λ ty, interp_type ty Σ) <$> σ.
+  Definition interp_list Σthis Σ (σ: list lang_ty) : list (interp Θ) :=
+    (λ ty, interp_type ty Σthis Σ) <$> σ
+  .
+
+  Lemma interp_list_lookup Σthis Σ σ k:
+    (interp_list Σthis Σ σ) !! k = (λ ty, interp_type ty Σthis Σ) <$> (σ !! k).
+  Proof. by rewrite /interp_list list_lookup_fmap. Qed.
+
+  (* TODO: find an explanation *)
+  Definition interp_tag_exact A (Σ: list (interp Θ)) :=
+    fixpoint (λ Σthis, interp_exact_tag interp_type A Σthis Σ).
 
   Section Unfold.
-    Variable Σ : list (interpO Θ).
+    Variable Σthis : interp Θ.
+    Variable Σ : list (interp Θ).
 
     (* Helper lemmas to control unfolding of some definitions *)
-
     Lemma interp_type_unfold (ty : lang_ty) :
-      interp_type ty Σ ≡ interp_type_pre interp_type ty Σ.
+      interp_type ty Σthis Σ ≡ interp_type_pre interp_type ty Σthis Σ.
     Proof.
       rewrite {1}/interp_type => v.
-      apply (fixpoint_unfold interp_type_pre ty Σ v).
+      apply (fixpoint_unfold interp_type_pre ty Σthis Σ v).
     Qed.
 
     Lemma interp_type_unfold_v (ty : lang_ty) (v: value):
-      interp_type ty Σ v ≡ interp_type_pre interp_type ty Σ v.
+      interp_type ty Σthis Σ v ≡ interp_type_pre interp_type ty Σthis Σ v.
     Proof.
       rewrite {1}/interp_type.
-      apply (fixpoint_unfold interp_type_pre ty Σ v).
+      apply (fixpoint_unfold interp_type_pre ty Σthis Σ v).
     Qed.
 
-    Lemma interp_type_unfold2 (ty : lang_ty) (v : value) :
-      interp_car (interp_type ty Σ) v ⊣⊢ interp_car (interp_type_pre interp_type ty Σ) v.
+    Lemma interp_tag_exact_unfold A v:
+      interp_tag_exact A Σ v ⊣⊢ interp_exact_tag interp_type A (interp_tag_exact A Σ) Σ v.
     Proof.
-      rewrite {1}/interp_type.
-      apply (fixpoint_unfold interp_type_pre ty Σ v).
+      rewrite {1}/interp_tag_exact.
+      apply (fixpoint_unfold (λ Σthis, interp_exact_tag interp_type A Σthis Σ)).
     Qed.
 
     (* #hyp *)
     Global Instance interp_type_persistent :
-    ∀ t v, Persistent (interp_type t Σ v).
+    ∀ t v, Persistent (interp_type t Σthis Σ v).
     Proof.
       move => t v.
       rewrite interp_type_unfold.
       by apply _.
     Qed.
 
-    Lemma interp_nonnull_unfold: interp_type NonNullT Σ ≡ interp_nonnull interp_type.
+    Lemma interp_nonnull_unfold:
+      interp_type NonNullT Σthis Σ ≡ interp_nonnull interp_type.
     Proof. by rewrite interp_type_unfold /= /interp_nonnull /=. Qed.
 
-    Lemma interp_mixed_unfold: interp_type MixedT Σ ≡ interp_mixed interp_type.
+    Lemma interp_mixed_unfold:
+      interp_type MixedT Σthis Σ ≡ interp_mixed interp_type.
     Proof. by rewrite interp_type_unfold /interp_mixed /=. Qed.
 
     Lemma interp_union_unfold A B:
-      interp_type (UnionT A B) Σ ≡ interp_union (interp_type A Σ) (interp_type B Σ).
+      interp_type (UnionT A B) Σthis Σ ≡
+      interp_union (interp_type A Σthis Σ) (interp_type B Σthis Σ).
     Proof.
       rewrite interp_type_unfold /= => v.
       iSplit; iIntros "[H | H]".
@@ -694,7 +979,8 @@ Section proofs.
     Qed.
 
     Lemma interp_inter_unfold A B:
-      interp_type (InterT A B) Σ ≡ interp_inter (interp_type A Σ) (interp_type B Σ).
+      interp_type (InterT A B) Σthis Σ ≡
+      interp_inter (interp_type A Σthis Σ) (interp_type B Σthis Σ).
     Proof.
       rewrite interp_type_unfold /interp_inter => v /=.
       iSplit; iIntros "[HL HR]".
@@ -703,20 +989,21 @@ Section proofs.
     Qed.
 
     Lemma interp_support_dynamic_unfold:
-      interp_type SupportDynT Σ ≡ interp_support_dynamic interp_type.
+      interp_type SupportDynT Σthis Σ ≡ interp_support_dynamic interp_type.
     Proof.  by rewrite interp_type_unfold. Qed.
 
     Lemma interp_dynamic_unfold:
-      interp_type DynamicT Σ ≡ interp_support_dynamic interp_type.
+      interp_type DynamicT Σthis Σ ≡ interp_support_dynamic interp_type.
     Proof.  by rewrite interp_type_unfold. Qed.
   End Unfold.
 
   Definition interp_tag_alt
-    (Σ : list (interp Θ))
     (C: tag)
+    (Σthis : interp Θ)
+    (Σ : list (interp Θ))
     : interp Θ :=
     Interp (
-      λ (w : value), (∃ ℓ t cdef tdef σ (Σt: list (interp Θ))
+      λ (w : value), (∃ ℓ t cdef tdef σ (Σt : list (interp Θ))
        (fields: stringmap ((visibility * lang_ty) * tag))
        (ifields: gmapO string (sem_typeO Θ)),
       ⌜w = LocV ℓ ∧
@@ -729,19 +1016,20 @@ Section proofs.
 
       □ ▷ interp_env_as_mixed Σt ∗
 
-      □ ▷ Σinterp Σt tdef.(constraints) ∗
+      □ ▷ Σinterp Σthis Σt tdef.(constraints) ∗
 
-      □ ▷ iForall3 interp_variance cdef.(generics) (interp_list Σt σ) Σ ∗
+      □ ▷ iForall3 interp_variance cdef.(generics) (interp_list Σthis Σt σ) Σ ∗
 
       ▷ (∀ f vis ty orig, ⌜has_field f t vis ty orig⌝ -∗
-          (ifields !! f ≡ Some (interp_car (interp_type ty Σt)))) ∗
+          (ifields !! f ≡ Some (interp_car (interp_type ty Σthis Σt)))) ∗
 
       (ℓ ↦ (t, ifields)))%I
     ).
 
   Definition interp_exact_tag_alt
-    (Σ : list (interp Θ))
     (C: tag)
+    (Σthis: interp Θ)
+    (Σ : list (interp Θ))
     : interp Θ :=
     Interp (
       λ (w : value), (∃ ℓ cdef (Σc: list (interp Θ))
@@ -755,29 +1043,29 @@ Section proofs.
 
       □ ▷ interp_env_as_mixed Σc ∗
 
-      □ ▷ Σinterp Σc cdef.(constraints) ∗
+      □ ▷ Σinterp Σthis Σc cdef.(constraints) ∗
 
       □ ▷ iForall3 interp_variance cdef.(generics) Σc Σ ∗
 
       ▷ (∀ f vis ty orig, ⌜has_field f C vis ty orig⌝ -∗
-          (ifields !! f ≡ Some (interp_car (interp_type ty Σc)))) ∗
+          (ifields !! f ≡ Some (interp_car (interp_type ty Σthis Σc)))) ∗
 
       (ℓ ↦ (C, ifields)))%I
     ).
 
-  Lemma interp_tag_equiv A Σ v:
+  Lemma interp_tag_equiv A Σthis Σ v:
     map_Forall (λ _cname, wf_cdef_parent pdefs) pdefs →
     ∀ adef, pdefs !! A = Some adef →
     length Σ = length adef.(generics) →
-    interp_tag interp_type Σ A v ⊣⊢
-    interp_tag_alt Σ A v.
+    interp_tag interp_type A Σthis Σ v ⊣⊢
+    interp_tag_alt A Σthis Σ v.
   Proof.
     move => hwfp adef hadef hlΣ.
     rewrite !interp_tag_unseal /interp_tag_def.
     rewrite /interp_fun !interp_car_simpl /=.
     rewrite /interp_env_as_mixed /Σinterp.
     iStartProof; iSplit; iIntros "#h".
-    - iDestruct "h" as (l t adef' tdef σ Σt fields ifields h) "[#hmixed [#hconstr [#hinst [#hdyn hloc]]]]".
+    - iDestruct "h" as (l t adef' tdef σ Σt fields ifields h) "(#hmixed & #hconstr & #hinst & #hdyn & hloc)".
       destruct h as (-> & hadef' & htdef & hlΣt &  hin & hfields & hidom); simplify_eq.
       iExists l, t, adef, tdef, σ, Σt, fields, ifields.
       iSplit => //.
@@ -794,7 +1082,7 @@ Section proofs.
       iModIntro; iNext.
       assert (hl1 : length Σ = length σ).
       { apply inherits_using_wf in hin => //.
-        destruct hin as (?&?&?&h).
+        destruct hin as (?&?&?&h&_).
         apply wf_tyI in h as (? & ? & ? & ?); simplify_eq.
         by rewrite hlΣ.
       }
@@ -802,7 +1090,11 @@ Section proofs.
       generalize (generics adef) => vs; clear => hl0 hl1.
       iClear "hmixed hdyn hloc".
       iInduction vs as [ | hd tl] "HI" forall (σ Σ hl0 hl1).
-      { by destruct σ; destruct Σ. }
+      { rewrite hl0 in hl1.
+        symmetry in hl1.
+        apply nil_length_inv in hl1 as ->.
+        by apply nil_length_inv in hl0 as ->.
+      }
       destruct σ as [ | t0 σ] => /=.
       { by rewrite hl1 in hl0. }
       destruct Σ as [ | i Σ] => //=.
@@ -813,7 +1105,7 @@ Section proofs.
       + iApply "HI" => //.
         iModIntro; iIntros (k v j0 j1 hk) "#h0 #h1".
         by iApply ("hinst" $! (S k)).
-    - iDestruct "h" as (l t adef' tdef σ Σt fields ifields h) "[#hmixed [#hconstr [#hinst [#hdyn hloc]]]]".
+    - iDestruct "h" as (l t adef' tdef σ Σt fields ifields h) "(#hmixed & #hconstr & #hinst & #hdyn & hloc)".
       destruct h as (-> & hadef' & htdef & hlΣt & hin & hfields & hidom); simplify_eq.
       iExists l, t, adef, tdef, σ, Σt, fields, ifields.
       iSplit => //.
@@ -830,7 +1122,7 @@ Section proofs.
       iModIntro; iNext.
       assert (hl1 : length Σ = length σ).
       { apply inherits_using_wf in hin => //.
-        destruct hin as (?&?&?&h).
+        destruct hin as (?&?&?&h&_).
         apply wf_tyI in h as (? & ? & ? & ?); simplify_eq.
         by rewrite hlΣ.
       }
@@ -856,12 +1148,12 @@ Section proofs.
       + by iApply ("HI" $! k).
   Qed.
 
-  Lemma interp_exact_tag_equiv A Σ v:
+  Lemma interp_exact_tag_equiv A Σthis Σ v:
     map_Forall (λ _cname, wf_cdef_parent pdefs) pdefs →
     ∀ adef, pdefs !! A = Some adef →
     length Σ = length adef.(generics) →
-    interp_exact_tag interp_type Σ A v ⊣⊢
-    interp_exact_tag_alt Σ A v.
+    interp_exact_tag interp_type A Σthis Σ v ⊣⊢
+    interp_exact_tag_alt A Σthis Σ v.
   Proof.
     move => hwfp adef hadef hlΣ.
     rewrite !interp_exact_tag_unseal /interp_exact_tag_def.
@@ -928,14 +1220,72 @@ Section proofs.
         * by iApply ("IH" $! Σc Σ).
   Qed.
 
+  Definition interp_class_alt t Σ : interp Θ :=
+    Interp (λ (w: value),
+     (∃ (Σthis : interp Θ),
+       □ ▷ (∀ v, Σthis v -∗ interp_tag_alt t Σthis Σ v) ∗
+       □ ▷ (interp_as_mixed Σthis) ∗
+       interp_tag_alt t Σthis Σ w))%I.
+
+  Lemma interp_class_equiv t Σ v:
+    map_Forall (λ _cname, wf_cdef_parent pdefs) pdefs →
+    ∀ def, pdefs !! t = Some def →
+    length Σ = length def.(generics) →
+    interp_class interp_type t Σ v ⊣⊢
+    interp_class_alt t Σ v.
+  Proof.
+    move => hwp def hdef hl.
+    rewrite /interp_class /interp_class_alt /=.
+    do 3 f_equiv.
+    { do 5 f_equiv.
+      by eapply interp_tag_equiv.
+    }
+    f_equiv.
+    { rewrite /interp_as_mixed /interp_inclusion.
+      do 5 f_equiv.
+      by rewrite interp_mixed_unfold.
+    }
+    by eapply interp_tag_equiv.
+  Qed.
+  
+  Definition interp_exact_class_alt t Σ : interp Θ :=
+    Interp (λ (w: value),
+     (∃ (Σthis : interp Θ),
+       □ ▷ (∀ v, Σthis v -∗ interp_exact_tag_alt t Σthis Σ v) ∗
+       □ ▷ (interp_as_mixed Σthis) ∗
+       interp_exact_tag_alt t Σthis Σ w))%I.
+
+  Lemma interp_exact_class_equiv t Σ v:
+    map_Forall (λ _cname, wf_cdef_parent pdefs) pdefs →
+    ∀ def, pdefs !! t = Some def →
+    length Σ = length def.(generics) →
+    interp_exact_class interp_type t Σ v ⊣⊢
+    interp_exact_class_alt t Σ v.
+  Proof.
+    move => hwp def hdef hl.
+    rewrite /interp_exact_class /interp_exact_class_alt /=.
+    do 3 f_equiv.
+    { do 5 f_equiv.
+      by eapply interp_exact_tag_equiv.
+    }
+    f_equiv.
+    { rewrite /interp_as_mixed /interp_inclusion.
+      do 5 f_equiv.
+      by rewrite interp_mixed_unfold.
+    }
+    by eapply interp_exact_tag_equiv.
+  Qed.
+
   Definition interp_sdt_alt : interp Θ :=
     Interp (λ (v: value),
-      (∃ A Σa adef, ⌜pdefs !! A = Some adef ∧
+      (∃ A Σthisa (Σa: list (interp Θ))  adef, ⌜pdefs !! A = Some adef ∧
         length Σa = length adef.(generics)⌝ ∗
-      □ ▷ (Σinterp Σa (Δsdt A)) ∗
+      □ ▷ (Σinterp Σthisa Σa (Δsdt A)) ∗
       □ ▷ (interp_env_as_mixed Σa) ∗
-      □ ▷ (Σinterp Σa adef.(constraints)) ∗
-      interp_tag_alt Σa A v))%I.
+      □ ▷ (Σinterp Σthisa Σa adef.(constraints)) ∗
+      □ ▷ (interp_as_mixed Σthisa) ∗
+      □ ▷ (∀ v, Σthisa v -∗ interp_tag_alt A Σthisa Σa v) ∗
+      interp_tag_alt A Σthisa Σa v))%I.
 
   Lemma interp_sdt_equiv v:
     map_Forall (λ _cname, wf_cdef_parent pdefs) pdefs →
@@ -944,21 +1294,30 @@ Section proofs.
   Proof.
     move => hwp.
     rewrite /interp_sdt /interp_sdt_alt /interp_variance /=.
-    do 6 f_equiv.
+    do 8 f_equiv.
     iSplit.
-    - iIntros "(%h0 & #h1 & #hmixed & #h3 & h4)".
+    - iIntros "(%h0 & #h1 & #hmixed & #h3 & #h4 & #h5 & #h6)".
       destruct h0 as [hadef hlen].
       iSplit; first done.
       iSplit; first done.
       iSplit.
       { iModIntro; iNext.
         iIntros (i phi hi w) "#hphi".
-        rewrite -(interp_type_unfold [] MixedT w).
+        rewrite -(interp_type_unfold a0 [] MixedT w).
         by iApply "hmixed".
       }
       iSplit; first done.
-      by rewrite interp_tag_equiv.
-    - iIntros "(%h0 & #h1 & #hmixed & #h3 & h4)".
+      iSplit.
+      { iModIntro; iNext.
+        iIntros (w) "#hw".
+        iSpecialize ("h5" $! w with "hw").
+        by rewrite interp_type_unfold_v.
+      }
+      iSplit; last by iApply interp_tag_equiv.
+      iModIntro; iNext; iIntros (w) "#hw".
+      iSpecialize ("h4" with "hw").
+      by iApply interp_tag_equiv.
+    - iIntros "(%h0 & #h1 & #hmixed & #h3 & #h4 & #h5 & #h6)".
       destruct h0 as [hadef hlen].
       iSplit; first done.
       iSplit; first done.
@@ -969,130 +1328,201 @@ Section proofs.
         by iApply "hmixed".
       }
       iSplit; first done.
-      by rewrite interp_tag_equiv.
+      iSplit.
+      { iModIntro; iNext; iIntros (w) "#hw".
+        iSpecialize ("h5" with "hw").
+        by iApply interp_tag_equiv.
+      }
+      iSplit.
+      { iModIntro; iNext.
+        iIntros (w) "#hw".
+        iSpecialize ("h4" $! w with "hw").
+        by rewrite interp_mixed_unfold.
+      }
+      by iApply interp_tag_equiv.
   Qed.
 
-  Lemma interp_tag_equivI (Σ0 Σ1: list (interp Θ)):
+  Lemma interp_tag_equivI Σthis (Σ0 Σ1: list (interp Θ)):
     Σ0 ≡ Σ1 →
-    ∀ A v, interp_tag interp_type Σ0 A v ≡ interp_tag interp_type Σ1 A v.
+    ∀ A v, interp_tag interp_type A Σthis Σ0 v ≡ interp_tag interp_type A Σthis Σ1 v.
   Proof.
     move => h A v.
     rewrite !interp_tag_unseal /interp_tag_def /interp_variance /=.
     by repeat f_equiv.
   Qed.
 
-  Lemma interp_tag_alt_equivI (Σ0 Σ1: list (interp Θ)):
+  Lemma interp_tag_alt_equivI Σthis (Σ0 Σ1: list (interp Θ)):
     map_Forall (λ _cname, wf_cdef_parent pdefs) pdefs →
     Σ0 ≡ Σ1 →
     ∀ A adef v,
     pdefs !! A = Some adef →
     length Σ0 = length adef.(generics) →
-    interp_tag_alt Σ0 A v ≡ interp_tag_alt Σ1 A v.
+    interp_tag_alt A Σthis Σ0 v ≡ interp_tag_alt A Σthis Σ1 v.
   Proof.
     move => hp h A adef v hadef hlen.
     rewrite -!(interp_tag_equiv A) //; first by rewrite interp_tag_equivI.
     by rewrite -hlen h.
   Qed.
 
-  Lemma interp_exact_tag_equivI (Σ0 Σ1: list (interp Θ)):
+  Lemma interp_exact_tag_equivI Σthis (Σ0 Σ1: list (interp Θ)):
     Σ0 ≡ Σ1 →
-    ∀ A v, interp_exact_tag interp_type Σ0 A v ≡ interp_exact_tag interp_type Σ1 A v.
+    ∀ A v, interp_exact_tag interp_type A Σthis Σ0 v ≡
+           interp_exact_tag interp_type A Σthis Σ1 v.
   Proof.
     move => h A v.
     rewrite !interp_exact_tag_unseal /interp_exact_tag_def /=.
     by do 29 f_equiv.
   Qed.
 
-  Lemma interp_exact_tag_alt_equivI (Σ0 Σ1: list (interp Θ)):
+  Lemma interp_exact_tag_alt_equivI Σthis (Σ0 Σ1: list (interp Θ)):
     map_Forall (λ _cname, wf_cdef_parent pdefs) pdefs →
     Σ0 ≡ Σ1 →
     ∀ A adef v,
     pdefs !! A = Some adef →
     length Σ0 = length adef.(generics) →
-    interp_exact_tag_alt Σ0 A v ≡ interp_exact_tag_alt Σ1 A v.
+    interp_exact_tag_alt A Σthis Σ0 v ≡
+    interp_exact_tag_alt A Σthis Σ1 v.
   Proof.
     move => hp h A adef v hadef hlen.
     rewrite -!(interp_exact_tag_equiv A) //; first by rewrite interp_exact_tag_equivI.
     by rewrite -hlen h.
   Qed.
 
-  Lemma interp_type_pre_equivI (Σ0 Σ1: list (interp Θ)):
+  Lemma interp_class_equivI (Σ0 Σ1: list (interp Θ)):
     Σ0 ≡ Σ1 →
-    ∀ ty v, interp_type_pre interp_type ty Σ0 v ≡ interp_type_pre interp_type ty Σ1 v.
+    ∀ A v, interp_class interp_type A Σ0 v ≡ interp_class interp_type A Σ1 v.
+  Proof.
+    move => h A v.
+    rewrite /interp_class /=.
+    do 3 f_equiv.
+    - do 5 f_equiv.
+      by rewrite interp_tag_equivI.
+    - by rewrite interp_tag_equivI.
+  Qed.
+
+  Lemma interp_class_alt_equivI (Σ0 Σ1: list (interp Θ)):
+    map_Forall (λ _cname, wf_cdef_parent pdefs) pdefs →
+    Σ0 ≡ Σ1 →
+    ∀ A adef v,
+    pdefs !! A = Some adef →
+    length Σ0 = length adef.(generics) →
+    interp_class_alt A Σ0 v ≡ interp_class_alt A Σ1 v.
+  Proof.
+    move => hp h A adef v hadef hlen.
+    rewrite -(interp_class_equiv A) //.
+    rewrite -(interp_class_equiv A) //; first by rewrite interp_class_equivI.
+    by rewrite -hlen h.
+  Qed.
+
+  Lemma interp_exact_class_equivI (Σ0 Σ1: list (interp Θ)):
+    Σ0 ≡ Σ1 →
+    ∀ A v, interp_exact_class interp_type A Σ0 v ≡
+           interp_exact_class interp_type A Σ1 v.
+  Proof.
+    move => h A v.
+    rewrite /interp_exact_class /=.
+    do 3 f_equiv.
+    - do 5 f_equiv.
+      by rewrite interp_exact_tag_equivI.
+    - by rewrite interp_exact_tag_equivI.
+  Qed.
+
+  Lemma interp_exact_class_alt_equivI (Σ0 Σ1: list (interp Θ)):
+    map_Forall (λ _cname, wf_cdef_parent pdefs) pdefs →
+    Σ0 ≡ Σ1 →
+    ∀ A adef v,
+    pdefs !! A = Some adef →
+    length Σ0 = length adef.(generics) →
+    interp_exact_class_alt A Σ0 v ≡ interp_exact_class_alt A Σ1 v.
+  Proof.
+    move => hp h A adef v hadef hlen.
+    rewrite -(interp_exact_class_equiv A) //.
+    rewrite -(interp_exact_class_equiv A) //; first by rewrite interp_exact_class_equivI.
+    by rewrite -hlen h.
+  Qed.
+
+  Lemma interp_type_pre_equivI Σthis (Σ0 Σ1: list (interp Θ)):
+    Σ0 ≡ Σ1 →
+    ∀ ty v, interp_type_pre interp_type ty Σthis Σ0 v ≡ interp_type_pre interp_type ty Σthis Σ1 v.
   Proof.
     move => h ty.
-    induction ty as [ | | | | exact_ C σ hi | | | A B hA hB | A B hA hB | i | | ] => v //=.
-    - assert (heq: go interp_type Σ0 <$> σ ≡ go interp_type Σ1 <$> σ).
+    induction ty as [ | | | | exact_ C σ hi | | | A B hA hB | A B hA hB | i | | | ] => v //=.
+    - assert (heq: go interp_type Σthis Σ0 <$> σ ≡ go interp_type Σthis Σ1 <$> σ).
       { apply list_fmap_equiv_ext => k ty hty w.
         rewrite Forall_lookup in hi.
         by eapply hi.
       }
       destruct exact_.
-      + by rewrite interp_exact_tag_equivI.
-      + by rewrite interp_tag_equivI.
+      + by rewrite interp_exact_class_equivI.
+      + by rewrite interp_class_equivI.
     - f_equiv; by eauto.
     - f_equiv; by eauto.
     - rewrite /interp_generic.
-      by rewrite h.
+      by rewrite /= h.
   Qed.
 
-  Lemma interp_type_equivI (Σ0 Σ1: list (interp Θ)):
+  Lemma interp_type_equivI Σthis (Σ0 Σ1: list (interp Θ)):
     Σ0 ≡ Σ1 →
-    ∀ ty v, interp_type ty Σ0 v ≡ interp_type ty Σ1 v.
+    ∀ ty v, interp_type ty Σthis Σ0 v ≡ interp_type ty Σthis Σ1 v.
   Proof.
     move => h ty v.
     rewrite !interp_type_unfold.
     by rewrite interp_type_pre_equivI.
   Qed.
 
-  Lemma interp_class_unfold Σ A σA v:
+  Lemma interp_class_unfold Σthis Σ A σA v:
     map_Forall (λ _cname, wf_cdef_parent pdefs) pdefs →
     wf_ty (ClassT true A σA) →
-    interp_type (ClassT false A σA) Σ v ⊣⊢
-    interp_tag_alt (interp_list Σ σA) A v.
+    interp_type (ClassT false A σA) Σthis Σ v ⊣⊢
+    interp_class_alt A (interp_list Σthis Σ σA) v.
   Proof.
     move => hwfp hwf.
     apply wf_tyI in hwf as (adef & ? & ? & ?); simplify_eq.
-    assert (hlen: length (interp_list Σ σA) = length (generics adef)).
+    assert (hlen: length (interp_list Σthis Σ σA) = length (generics adef)).
     { by rewrite /interp_list map_length. }
-    rewrite -interp_tag_equiv // interp_type_unfold /=.
-    apply interp_tag_equivI.
+    rewrite -interp_class_equiv // interp_type_unfold /=.
+    apply interp_class_equivI.
     rewrite /interp_list.
     apply list_fmap_equiv_ext => ? ty ? w.
     by rewrite interp_type_unfold.
   Qed.
 
-  Lemma interp_class_unfold_exact Σ A σA v:
+  Lemma interp_exact_class_unfold Σthis Σ A σA v:
     map_Forall (λ _cname, wf_cdef_parent pdefs) pdefs →
     wf_ty (ClassT true A σA) →
-    interp_type (ClassT true A σA) Σ v ⊣⊢
-    interp_exact_tag_alt (interp_list Σ σA) A v.
+    interp_type (ClassT true A σA) Σthis Σ v ⊣⊢
+    interp_exact_class_alt A (interp_list Σthis Σ σA) v.
   Proof.
     move => hwfp hwf.
     apply wf_tyI in hwf as (adef & ? & ? & ?); simplify_eq.
-    assert (hlen: length (interp_list Σ σA) = length (generics adef)).
+    assert (hlen: length (interp_list Σthis Σ σA) = length (generics adef)).
     { by rewrite /interp_list map_length. }
-    rewrite -interp_exact_tag_equiv // interp_type_unfold /=.
-    apply interp_exact_tag_equivI.
+    rewrite -interp_exact_class_equiv // interp_type_unfold /=.
+    apply interp_exact_class_equivI.
     rewrite /interp_list.
     apply list_fmap_equiv_ext => ? ty ? w.
     by rewrite interp_type_unfold.
   Qed.
 
-  Lemma interp_generic_unfold Σ k v:
-    interp_type (GenT k) Σ v ⊣⊢
+  Lemma interp_generic_unfold Σthis Σ k v:
+    interp_type (GenT k) Σthis Σ v ⊣⊢
     interp_generic Σ k v.
-  Proof.  by rewrite interp_type_unfold /=. Qed.
+  Proof. by rewrite interp_type_unfold /=. Qed.
 
-  Lemma interp_type_subst Σ ty σ v:
+  Lemma interp_this_unfold Σthis Σ v:
+    interp_type ThisT Σthis Σ v ⊣⊢ Σthis v.
+  Proof. by rewrite interp_type_unfold /=. Qed.
+
+  Lemma interp_type_subst Σthis Σ ty σ v:
     bounded (length σ) ty →
-    interp_type (subst_ty σ ty) Σ v ≡
-    interp_type ty (interp_list Σ σ) v.
+    interp_type (subst_ty σ ty) Σthis Σ v ≡
+    interp_type ty Σthis (interp_list Σthis Σ σ) v.
   Proof.
     move => hbounded.
     rewrite !interp_type_unfold; revert v.
-    induction ty as [ | | | | exact_ C σC hi | | | A B hA hB | A B hA hB | i | | ] => //= v.
-    - assert (heq: go interp_type Σ <$> (subst_ty σ <$> σC) ≡ go interp_type (interp_list Σ σ) <$> σC).
+    induction ty as [ | | | | exact_ C σC hi | | | A B hA hB | A B hA hB | i | | | ] => //= v.
+    - assert (heq: go interp_type Σthis Σ <$> (subst_ty σ <$> σC) ≡
+                   go interp_type Σthis (interp_list Σthis Σ σ) <$> σC).
       { rewrite -list_fmap_compose.
         apply list_fmap_equiv_ext => ? ty hin w.
         apply elem_of_list_lookup_2 in hin.
@@ -1103,10 +1533,8 @@ Section proofs.
         by apply hbounded.
       }
       destruct exact_.
-      + rewrite !interp_exact_tag_unseal /interp_exact_tag_def /=.
-        by do 29 f_equiv.
-      + rewrite !interp_tag_unseal /interp_tag_def /= /interp_variance.
-        by do 35 f_equiv.
+      + by apply interp_exact_class_equivI.
+      + by apply interp_class_equivI.
     - apply boundedI in hbounded as [??]; by rewrite hA // hB.
     - apply boundedI in hbounded as [??]; by rewrite hA // hB.
     - rewrite /interp_generic list_lookup_fmap.
@@ -1117,14 +1545,168 @@ Section proofs.
         by lia.
   Qed.
 
-  Lemma interp_type_pre_app ty: ∀ Σ0 Σ1,
-    bounded (length Σ0) ty →
-    interp_type_pre interp_type ty Σ0 ≡
-    interp_type_pre interp_type ty (Σ0 ++ Σ1).
+  Lemma interp_type_no_this Σ ty v (Σ0 Σ1: interp Θ):
+    no_this ty → interp_type ty Σ0 Σ v ≡ interp_type ty Σ1 Σ v.
   Proof.
-    induction ty as [ | | | | exact_ A σ hi | | | A B hA hB | A B hA hB | i | | ]
+    rewrite !interp_type_unfold; revert v.
+    induction ty as [ | | | | exact_ C σC hi | | | A B hA hB | A B hA hB | i | | | ] => //= v hnothis.
+    - assert (heq: go interp_type Σ0 Σ <$> σC ≡
+                   go interp_type Σ1 Σ <$> σC).
+      { apply list_fmap_equiv_ext => ? ty hin w.
+        apply elem_of_list_lookup_2 in hin.
+        rewrite Forall_forall in hi.
+        apply hi with (v := w) in hin; first by rewrite hin.
+        apply forallb_True in hnothis.
+        rewrite Forall_forall in hnothis.
+        by apply hnothis.
+      }
+      destruct exact_.
+      + by apply interp_exact_class_equivI.
+      + by apply interp_class_equivI.
+    - apply andb_prop_elim in hnothis as [h0 h1].
+      apply hA with v in h0.
+      apply hB with v in h1.
+      by f_equiv.
+    - apply andb_prop_elim in hnothis as [h0 h1].
+      apply hA with v in h0.
+      apply hB with v in h1.
+      by f_equiv.
+  Qed.
+
+  Lemma interp_list_no_this Σ σ (Σ0 Σ1: interp Θ):
+    Forall no_this σ → interp_list Σ0 Σ σ ≡ interp_list Σ1 Σ σ.
+  Proof.
+    induction σ as [ | ty σ hi]; first done.
+    case/Forall_cons => hty hσ /=.
+    f_equiv; last by apply hi.
+    move => v.
+    by apply interp_type_no_this.
+  Qed.
+
+  Lemma interp_type_subst_this_exact t tdef Σthis Σ ty v:
+    map_Forall (λ _cname, wf_cdef_parent pdefs) pdefs →
+    map_Forall (λ _cname, wf_cdef_constraints_no_this) pdefs →
+    pdefs !! t = Some tdef →
+    length Σ = length tdef.(generics) →
+    interp_type (subst_this (ClassT true t (gen_targs (length Σ))) ty) Σthis Σ v ≡
+    interp_type ty (interp_tag_exact t Σ) Σ v.
+    else interp_type ty (interp_tag t Σ
+  Proof.
+    move => hwp hwfno htdef hlen.
+    rewrite !interp_type_unfold; revert v.
+    induction ty as [ | | | | C σC hi | | | A B hA hB | A B hA hB | i | | | ] => //= v.
+    - assert (htag: ∀ Σthis0 w,
+        interp_tag interp_type C Σthis0
+          (go interp_type Σthis Σ <$> (subst_this (ClassT t (gen_targs (length Σ))) <$> σC)) w
+        ≡
+        interp_tag interp_type C Σthis0
+          (go interp_type (interp_tag_exact t Σ) Σ <$> σC) w).
+      { move => Σthis0 w.
+        rewrite !interp_tag_unseal /interp_tag_def /= /interp_variance.
+        do 34 f_equiv.
+        rewrite -list_fmap_compose.
+        apply list_equiv_lookup; simpl.
+        apply list_fmap_equiv_ext => ? ty hin w0.
+        rewrite Forall_forall in hi.
+        apply elem_of_list_lookup_2 in hin.
+        apply hi with (v := w0) in hin.
+        by rewrite hin.
+      }
+      do 3 f_equiv.
+      { do 5 f_equiv.
+        by apply htag.
+      }
+      f_equiv.
+      by apply htag.
+    - by rewrite hA hB.
+    - by rewrite hA hB.
+    - rewrite interp_tag_exact_unfold.
+      iSplit.
+      + iIntros "htag".
+        iDestruct "htag" as (Σthis0) "(#hcond & #htmixed & #htag)".
+        rewrite (interp_tag_unseal _ _ (interp_tag_exact t Σ)) {2}interp_tag_unseal.
+        rewrite /interp_tag_def /interp_fun !interp_car_simpl.
+        iDestruct "htag" as (l t0 cdef t0def σ Σt fields ifields h) "(#hmixed & #hconstr & #hinst & hfields & hloc)".
+        destruct h as (-> & hcdef & ht0def & hlΣt & hinherits & hfields & hdom).
+        iExists l, t0, cdef, t0def, σ, Σt, fields, ifields.
+        simplify_eq.
+        iSplitR; first done.
+        iSplitR.
+        { iModIntro; iNext; iIntros (i ii heq w0) "hii".
+          iSpecialize ("hmixed" $! i ii heq w0 with "hii").
+          iDestruct (interp_mixed_unfold Σthis0 [] w0) as "[hm0 ?]".
+          iDestruct (interp_mixed_unfold (interp_tag_exact t Σ) [] w0) as "[? hm3]".
+          iDestruct ("hm0" with "hmixed") as "hm".
+          by iApply "hm3".
+        }
+        iSplitR.
+        { iModIntro; iNext; iIntros (i c heq w0) "hc".
+          assert (hno: no_this_constraint c).
+          { apply hwfno in ht0def.
+            rewrite /wf_cdef_constraints_no_this Forall_lookup in ht0def.
+            by apply ht0def in heq.
+          }
+          destruct hno as [].
+          iAssert (interp_type c.1 Σthis0 Σt w0) with "[hc]" as "hc".
+          { by iApply interp_type_no_this. }
+          iSpecialize ("hconstr" $! i c heq w0 with "hc").
+          by iApply interp_type_no_this.
+        }
+        iSplitR.
+        { iModIntro; iNext.
+          iIntros (k var i0 i1 hk) "#h0 #h1".
+          rewrite !list_lookup_fmap /= !option_equivI /=.
+          destruct (σ !! k) as [ty0 | ] eqn:hty0; last done.
+          simpl.
+          destruct (Σ !! k) as [ik | ] eqn:hik; last done.
+          iSpecialize ("hinst" $! k var (interp_type ty0 Σthis0 Σt) (interp_generic Σ k) hk).
+          assert (k < length Σ) by by apply lookup_lt_Some in hik.
+          rewrite !list_lookup_fmap hty0 /=.
+          rewrite lookup_seq_lt //=.
+          iSpecialize ("hinst" $! _ _).
+          apply inherits_using_wf in hinherits => //.
+          destruct hinherits as (? & ? & _ & _ & hFno).
+          rewrite Forall_lookup in hFno.
+          apply hFno in hty0.
+          rewrite /interp_generic /= hik /=.
+          destruct var; iIntros (w0); simpl.
+          - iDestruct ("hinst" $! w0) as "[hi0 hi1]".
+            iSplit; iIntros "#hw0".
+            + iRewrite -"h1".
+              iApply "hi0".
+              rewrite (interp_type_no_this _ _ _ Σthis0 (interp_tag_exact t Σ)); last done.
+              by iRewrite "h0".
+            + iRewrite -"h0".
+              rewrite (interp_type_no_this _ _ _ (interp_tag_exact t Σ) Σthis0); last done.
+              iApply "hi1".
+              by iRewrite "h1".
+          - iSpecialize ("hinst" $! w0).
+            iIntros "#hw0".
+            iRewrite -"h1".
+            iApply "hinst".
+            rewrite (interp_type_no_this _ _ _ Σthis0 (interp_tag_exact t Σ)); last done.
+            by iRewrite "h0".
+          - iSpecialize ("hinst" $! w0).
+            iIntros "#hw0".
+            iRewrite -"h0".
+            rewrite (interp_type_no_this _ _ _ (interp_tag_exact t Σ) Σthis0); last done.
+            iApply "hinst".
+            by iRewrite "h1".
+        }
+        iSplit; last done.
+        iNext; iIntros (f vis ty orig hf).
+
+
+  Qed.
+
+  Lemma interp_type_pre_app ty Σthis: ∀ (Σ0 Σ1: list (interp Θ)),
+    bounded (length Σ0) ty →
+    interp_type_pre interp_type ty Σthis Σ0 ≡
+    interp_type_pre interp_type ty Σthis (Σ0 ++ Σ1).
+  Proof.
+    induction ty as [ | | | | exact_ A σ hi | | | A B hA hB | A B hA hB | i | | | ]
         => Σ0 Σ1 hb w //=.
-    - assert (heq: go interp_type Σ0 <$> σ ≡ go interp_type (Σ0 ++ Σ1) <$> σ).
+    - assert (heq: go interp_type Σthis Σ0 <$> σ ≡ go interp_type Σthis (Σ0 ++ Σ1) <$> σ).
       { rewrite Forall_lookup in hi.
         apply list_fmap_equiv_ext => k ty hin w0.
         apply hi with (Σ0 := Σ0) (Σ1 := Σ1) in hin; first done.
@@ -1133,10 +1715,8 @@ Section proofs.
         by eauto.
       }
       destruct exact_.
-      + rewrite !interp_exact_tag_unseal /interp_exact_tag_def /interp_fun !interp_car_simpl.
-        by do 29 f_equiv.
-      + rewrite !interp_tag_unseal /interp_tag_def /interp_fun !interp_car_simpl.
-        by do 35 f_equiv.
+      + by apply interp_exact_class_equivI.
+      + by apply interp_class_equivI.
     - apply boundedI in hb as [h1 h2].
       f_equiv.
       + by apply hA with (Σ1 := Σ1) in h1.
@@ -1149,32 +1729,31 @@ Section proofs.
       by rewrite /interp_generic lookup_app_l.
   Qed.
 
-  Lemma interp_type_app ty: ∀ Σ0 Σ1,
+  Lemma interp_type_app ty Σthis: ∀ (Σ0 Σ1: list (interp Θ)),
     bounded (length Σ0) ty →
-    interp_type ty Σ0 ≡
-    interp_type ty (Σ0 ++ Σ1).
+    interp_type ty Σthis Σ0 ≡
+    interp_type ty Σthis (Σ0 ++ Σ1).
   Proof.
     move => Σ0 Σ1 hb v.
     by rewrite !interp_type_unfold interp_type_pre_app.
   Qed.
 
-  Lemma interp_type_pre_lift ty: ∀ Σ0 Σ1,
-    interp_type_pre interp_type (lift_ty (length Σ0) ty) (Σ0 ++ Σ1) ≡
-    interp_type_pre interp_type ty Σ1.
+  Lemma interp_type_pre_lift ty Σthis: ∀ (Σ0 Σ1: list (interp Θ)),
+    interp_type_pre interp_type (lift_ty (length Σ0) ty) Σthis (Σ0 ++ Σ1) ≡
+    interp_type_pre interp_type ty Σthis Σ1.
   Proof.
-    induction ty as [ | | | | exact_ A σ hi | | | A B hA hB | A B hA hB | i | | ]
+    induction ty as [ | | | | exact_ A σ hi | | | A B hA hB | A B hA hB | i | | | ]
         => Σ0 Σ1 w //=.
-    - assert (heq: go interp_type (Σ0 ++ Σ1) <$> (lift_ty (length Σ0) <$> σ) ≡ go interp_type Σ1 <$> σ).
+    - assert (heq: go interp_type Σthis (Σ0 ++ Σ1) <$> (lift_ty (length Σ0) <$> σ) ≡
+                   go interp_type Σthis Σ1 <$> σ).
       { rewrite Forall_lookup in hi.
         rewrite -list_fmap_compose.
         apply list_fmap_equiv_ext => k ty hin w0.
         by apply hi with (Σ0 := Σ0) (Σ1 := Σ1) in hin.
       }
       destruct exact_.
-      + rewrite !interp_exact_tag_unseal /interp_exact_tag_def /interp_fun !interp_car_simpl.
-        by do 29 f_equiv.
-      + rewrite !interp_tag_unseal /interp_tag_def /interp_fun !interp_car_simpl.
-        by do 35 f_equiv.
+      + by apply interp_exact_class_equivI.
+      + by apply interp_class_equivI.
     - f_equiv.
       + by apply hA with (Σ1 := Σ1).
       + by apply hB with (Σ1 := Σ1).
@@ -1185,39 +1764,39 @@ Section proofs.
       by rewrite Nat.add_sub.
   Qed.
 
-  Lemma interp_type_lift ty: ∀ Σ0 Σ1,
-    interp_type (lift_ty (length Σ0) ty) (Σ0 ++ Σ1) ≡
-    interp_type ty Σ1.
+  Lemma interp_type_lift ty Σthis: ∀ Σ0 Σ1,
+    interp_type (lift_ty (length Σ0) ty) Σthis (Σ0 ++ Σ1) ≡
+    interp_type ty Σthis Σ1.
   Proof.
     move => Σ0 Σ1 v.
     by rewrite !interp_type_unfold interp_type_pre_lift.
   Qed.
 
-  Lemma Σinterp_lift Δ: ∀ Σ0 Σ1,
-    Σinterp (Σ0 ++ Σ1) (lift_constraints (length Σ0) Δ) ≡
-    Σinterp Σ1 Δ.
+  Lemma Σinterp_lift Δ Σthis: ∀ Σ0 Σ1,
+    Σinterp Σthis (Σ0 ++ Σ1) (lift_constraints (length Σ0) Δ) ≡
+    Σinterp Σthis Σ1 Δ.
   Proof.
     iIntros (Σ0 Σ1).
     iSplit; iIntros "hΣ"; iIntros (i c heq v) "#h".
-    - rewrite -(interp_type_lift c.2 Σ0 Σ1).
+    - rewrite -(interp_type_lift c.2 Σthis Σ0 Σ1).
       assert (heq2: (lift_constraints (length Σ0) Δ) !! i = Some (lift_constraint (length Σ0) c)).
       { by rewrite /lift_constraints list_lookup_fmap heq. }
       iApply ("hΣ" $! i (lift_constraint (length Σ0) c) heq2 v).
       by rewrite interp_type_lift.
     - apply list_lookup_fmap_inv in heq as [c0 [-> hc]].
-      rewrite !interp_type_lift.
+      rewrite !interp_type_lift //.
       by iApply ("hΣ" $! i).
   Qed.
 
-  Lemma iForall3_interp_equivI_l (Σ0 Σ1 : list (interp Θ)):
+  Lemma iForall3_interp_equivI_l (Σ0 Σ1: list (interp Θ)):
     Σ0 ≡ Σ1 →
-    ∀ vs Σ,
+    ∀ vs (Σ: list (interp Θ)),
     iForall3 interp_variance vs Σ0 Σ ≡ iForall3 interp_variance vs Σ1 Σ.
   Proof.
-    move => heq vs.
+    move => heq vs Σ.
     assert (hl: length Σ0 = length Σ1) by by rewrite heq.
-    move : Σ0 Σ1 heq hl.
-    induction vs as [ | v vs hi] => Σ0 Σ1 heq hl Σ.
+    move : Σ Σ0 Σ1 heq hl.
+    induction vs as [ | v vs hi] => Σ Σ0 Σ1 heq hl.
     { by destruct Σ0; destruct Σ1; destruct Σ. }
     destruct Σ0 as [ | i0 Σ0] => //=.
     { symmetry in hl.
@@ -1230,18 +1809,18 @@ Section proofs.
     f_equiv.
     - rewrite /interp_variance.
       by repeat f_equiv.
-    - by rewrite (hi _ _ h1 hl Σ).
+    - by rewrite (hi Σ _ _ h1 hl).
   Qed.
 
-  Lemma iForall3_interp_equivI_r (Σ0 Σ1 : list (interp Θ)):
+  Lemma iForall3_interp_equivI_r (Σ0 Σ1: list (interp Θ)):
     Σ0 ≡ Σ1 →
-    ∀ vs Σ,
+    ∀ vs (Σ: list (interp Θ)),
     iForall3 interp_variance vs Σ Σ0 ≡ iForall3 interp_variance vs Σ Σ1.
   Proof.
-    move => heq vs.
+    move => heq vs Σ.
     assert (hl: length Σ0 = length Σ1) by by rewrite heq.
-    move : Σ0 Σ1 heq hl.
-    induction vs as [ | v vs hi] => Σ0 Σ1 heq hl Σ.
+    move : Σ Σ0 Σ1 heq hl.
+    induction vs as [ | v vs hi] => Σ Σ0 Σ1 heq hl.
     { by destruct Σ0; destruct Σ1; destruct Σ. }
     destruct Σ0 as [ | i0 Σ0] => //=.
     { symmetry in hl.
@@ -1254,63 +1833,67 @@ Section proofs.
     f_equiv.
     - rewrite /interp_variance.
       by repeat f_equiv.
-    - by rewrite (hi _ _ h1 hl Σ).
+    - by rewrite (hi Σ _ _ h1 hl).
   Qed.
 
-  Lemma interp_type_rigid Σ0 Σ1 t:
+  Lemma interp_type_rigid Σthis (Σ0 Σ1 : list (interp Θ)) t:
     map_Forall (λ _ : string, wf_cdef_parent pdefs) pdefs →
     wf_ty (ClassT true t (map GenT (seq (length Σ0) (length Σ1)))) →
-    interp_tag interp_type Σ1 t ≡
-    interp_type (ClassT false t (map GenT (seq (length Σ0) (length Σ1)))) (Σ0 ++ Σ1).
+    interp_class interp_type t Σ1 ≡
+    interp_type (ClassT false t (map GenT (seq (length Σ0) (length Σ1)))) Σthis (Σ0 ++ Σ1).
   Proof.
     move => hp hwf v.
     assert (h0 := hwf).
     apply wf_tyI in h0 as (? & ? & hlen & ?).
     rewrite map_length seq_length in hlen.
-    rewrite interp_tag_equiv //.
-    rewrite interp_class_unfold => //.
-    rewrite /interp_tag_alt /=.
-    do 18 f_equiv.
-    do 4 f_equiv.
-    assert (h : interp_list (Σ0 ++ Σ1) (map GenT (seq (length Σ0) (length Σ1))) ≡ Σ1).
-    { rewrite /interp_list.
-      apply list_equiv_lookup => k.
+    assert (h:
+      (λ ty, interp_type ty Σthis (Σ0 ++ Σ1)) <$> map GenT (seq (length Σ0) (length Σ1)) ≡ Σ1
+    ).
+    { apply list_equiv_lookup => k /=.
       rewrite !list_lookup_fmap.
       destruct (Σ1 !! k) as [ϕ | ] eqn:heq; last first.
       { rewrite heq.
         apply lookup_ge_None_1 in heq.
-        by rewrite lookup_seq_ge.
+        by rewrite lookup_seq_ge /=.
       }
       rewrite lookup_seq_lt; last first.
       { apply mk_is_Some in heq.
         by apply lookup_lt_is_Some_1 in heq.
       }
-      rewrite /= heq; f_equiv => w.
-      rewrite interp_generic_unfold /interp_generic lookup_app_r; last by lia.
-      replace (length Σ0 + k - length Σ0) with k by lia.
+      rewrite heq /=.
+      f_equiv => w.
+      rewrite interp_generic_unfold /interp_generic /= lookup_app_r; last by apply Nat.le_add_r.
+      rewrite Nat.sub_add'.
       by rewrite heq.
     }
+    rewrite interp_class_equiv //=.
+    rewrite interp_class_unfold; [ | done | done].
+    rewrite /interp_class_alt /=.
+    do 3 f_equiv.
+    { do 27 f_equiv.
+      by rewrite (iForall3_interp_equivI_r _ _ h).
+    }
+    do 22 f_equiv.
     by rewrite (iForall3_interp_equivI_r _ _ h).
   Qed.
 
-  Lemma iForall3_interp_gen_targs vs n Σ:
+  Lemma iForall3_interp_gen_targs vs n Σthis Σ:
     length vs = n →
     length Σ = n →
-    ⊢ iForall3 interp_variance vs (interp_list Σ (gen_targs n)) Σ.
+    ⊢ iForall3 interp_variance vs (interp_list Σthis Σ (gen_targs n)) Σ.
   Proof.
     move => hl0 hl1.
-    assert (heq: interp_list Σ (gen_targs n) ≡ Σ).
-    { rewrite /interp_list.
+    assert (heq: interp_list Σthis Σ (gen_targs n) ≡ Σ).
+    { rewrite /interp_list /=.
       apply list_equiv_lookup => k.
       destruct (Σ !! k) as [i | ] eqn:hi.
-      - rewrite !list_lookup_fmap hi !lookup_seq_lt //=.
+      - rewrite !list_lookup_fmap !lookup_seq_lt //=.
         { f_equiv => w.
           by rewrite !interp_generic_unfold /interp_generic /= hi.
         }
         apply lookup_lt_Some in hi.
         by lia.
-      - rewrite hi.
-        apply lookup_ge_None_1 in hi.
+      - apply lookup_ge_None_1 in hi.
         rewrite /gen_targs !list_lookup_fmap /= lookup_seq_ge //.
         by lia.
     }
@@ -1320,7 +1903,7 @@ Section proofs.
   Qed.
 
   Lemma iForall3_interp_trans vs:
-    ∀ Σ0 Σ1 Σ2,
+    ∀ (Σ0 Σ1 Σ2: list (interp Θ)),
     iForall3 interp_variance vs Σ0 Σ1 -∗
     iForall3 interp_variance vs Σ1 Σ2 -∗
     iForall3 interp_variance vs Σ0 Σ2.
@@ -1345,7 +1928,7 @@ Section proofs.
     - by iApply (hi with "h01 h11").
   Qed.
 
-  Lemma neg_interp_variance vs Σ0 Σ1:
+  Lemma neg_interp_variance vs (Σ0 Σ1: list (interp Θ)):
     iForall3 interp_variance vs Σ0 Σ1 -∗
     iForall3 interp_variance (neg_variance <$> vs) Σ1 Σ0.
   Proof.
@@ -1363,206 +1946,252 @@ Section proofs.
   Lemma interp_with_mono ty vs:
     map_Forall (λ _ : string, wf_cdef_mono) pdefs →
     map_Forall (λ _ : string, wf_cdef_parent pdefs) pdefs →
-    ∀ Σ0 Σ1,
+    ∀ (Σ0 Σ1: list (interp Θ)) (Σthis: interp Θ),
     mono vs ty →
     wf_ty ty →
     □ iForall3 interp_variance vs Σ0 Σ1 -∗
     ∀ v,
-    interp_type ty Σ0 v -∗ interp_type ty Σ1 v.
+    interp_type ty Σthis Σ0 v -∗ interp_type ty Σthis Σ1 v.
   Proof.
     move => ??.
-    iIntros (Σ0 Σ1 hmono hwf) "#h".
-    iInduction ty as [ | | | | exact_ C σC hi | | | A B hA hB | A B hA hB | i | | ]
-        "IHty" forall (Σ0 Σ1 vs hmono) "h"; iIntros (v); rewrite !interp_type_unfold //=.
+    iIntros (Σ0 Σ1 Σthis hmono hwf) "#h".
+    iInduction ty as [ | | | | exact_ C σC hi | | | A B hA hB | A B hA hB | i | | | ]
+        "IHty" forall (Σ0 Σ1 Σthis vs hmono) "h"; iIntros (v); rewrite !interp_type_unfold /=.
+    - by iIntros.
+    - by iIntros.
+    - by iIntros.
     - by iIntros.
     - destruct exact_.
-      + rewrite !interp_exact_tag_unseal /interp_exact_tag_def /interp_fun !interp_car_simpl.
-        iIntros "htag".
-        iDestruct "htag" as (l cdef Σc fields ifields h) "(#hmixed & #hconstr & #hinst & #hfields & hloc)".
-        destruct h as (-> & hcdef & hfields & hdom).
-        iExists l, cdef, Σc, fields, ifields.
-        iSplitR; first done.
-        iSplitR; first done.
-        iSplitR; first done.
-        iSplitR; last by iSplit.
-        iModIntro; iNext.
-        iDestruct (iForall3_length with "h") as "%hlen".
-        destruct hlen as [hl0 hl1].
-        iIntros (k v i0 i1 hk) "#h0 #h1".
-        rewrite !list_lookup_fmap.
-        destruct (σC !! k) as [t1 | ] eqn:ht1; last first.
-        { by rewrite !option_equivI. }
-        iSpecialize ("hinst" $! k v i0 (go interp_type Σ0 t1) hk with "h0").
-        rewrite /= !option_equivI.
-        iDestruct (neg_interp_variance with "h") as "hneg".
-        rewrite /interp_variance.
-        assert (hwf1: wf_ty t1).
-        { apply wf_tyI in hwf as (? & ? & ? & hwf); simplify_eq.
-          rewrite Forall_lookup in hwf.
-          by apply hwf with k.
-        }
-        iAssert (Some (go interp_type Σ0 t1) ≡ Some (go interp_type Σ0 t1))%I as "heq1"; first done.
-        rewrite !list_lookup_fmap /= ht1 !option_equivI.
-        iSpecialize ("hinst" with "heq1").
-        destruct v.
-        * assert (hmono0: mono vs t1).
-          { elim/mono_classI : hmono => cdef' hcdef' hnotcontra hnotcov; simplify_eq.
-            by apply hnotcontra with k Invariant.
+      + iAssert (∀ Σthis0 w0,
+          interp_exact_tag interp_type C Σthis0 (go interp_type Σthis Σ0 <$> σC) w0 -∗
+          interp_exact_tag interp_type C Σthis0 (go interp_type Σthis Σ1 <$> σC) w0)%I as "H".
+          { iIntros (Σthis0 w0) "#htag".
+            rewrite !interp_exact_tag_unseal /interp_exact_tag_def /interp_fun !interp_car_simpl.
+            iDestruct "htag" as (l cdef Σc fields ifields h) "(#hmixed & #hconstr & #hinst & hfields & hloc)".
+            destruct h as (-> & hcdef & hlΣc & hfields & hdom).
+            iExists l, cdef, Σc, fields, ifields.
+            iSplitR; first done.
+            iSplitR.
+            { iModIntro; iNext; iIntros (i ii heq w0) "hii".
+              iSpecialize ("hmixed" $! i ii heq w0 with "hii").
+              iClear "IHty h hinst".
+              iDestruct (interp_mixed_unfold Σthis0 [] w0) as "[hm0 ?]".
+              iDestruct (interp_mixed_unfold Σthis0 [] w0) as "[? hm3]".
+              iDestruct ("hm0" with "hmixed") as "hm".
+              by iApply "hm3".
+            }
+            iSplitR.
+            { iModIntro; iNext; iIntros (i c heq w0) "hc".
+              by iSpecialize ("hconstr" $! i c heq w0 with "hc").
+            }
+            iSplitR; last by iSplit.
+            iModIntro; iNext.
+            iDestruct (iForall3_length with "h") as "%hlen".
+            destruct hlen as [hl0 hl1].
+            iIntros (k var i0 i1 hk) "h0 h1".
+            rewrite !list_lookup_fmap.
+            destruct (σC !! k) as [t1 | ] eqn:ht1; last first.
+            { by rewrite !option_equivI. }
+            iSpecialize ("hinst" $! k var i0 (go interp_type Σthis Σ0 t1) hk with "h0").
+            rewrite /= !option_equivI.
+            iDestruct (neg_interp_variance with "h") as "hneg".
+            rewrite /interp_variance.
+            assert (hwf1: wf_ty t1).
+            { apply wf_tyI in hwf as (? & ? & ? & hwf); simplify_eq.
+              rewrite Forall_lookup in hwf.
+              by apply hwf with k.
+            }
+            iAssert (Some (go interp_type Σthis Σ0 t1) ≡ Some (go interp_type Σthis Σ0 t1))%I as "heq1"; first done.
+            rewrite !list_lookup_fmap /= ht1 !option_equivI.
+            iSpecialize ("hinst" with "heq1").
+            destruct var.
+            * assert (hmono0: mono vs t1).
+              { elim/mono_classI : hmono => cdef' hcdef' hnotcontra hnotcov; simplify_eq.
+                by apply hnotcontra with k Invariant.
+              }
+              assert (hmono1: mono (neg_variance <$> vs) t1).
+              { elim/mono_classI : hmono => cdef' hcdef' hnotcontra hnotcov; simplify_eq.
+                by apply hnotcov with k Invariant.
+              }
+              iAssert (□ ∀ w, interp_type t1 Σthis Σ0 w -∗ interp_type t1 Σthis Σ1 w)%I as "#hc0".
+              { iDestruct (big_sepL_lookup with "IHty") as "#hk"; first by exact ht1.
+                by iApply ("hk" $! hwf1 Σ0 Σ1 _ _ hmono0 with "h").
+              }
+              iAssert (□ ∀ w, interp_type t1 Σthis Σ1 w -∗ interp_type t1 Σthis Σ0 w)%I as "#hc1".
+              { iDestruct (big_sepL_lookup with "IHty") as "#hk"; first by exact ht1.
+                by iApply ("hk" $! hwf1 Σ1 Σ0 _ _ hmono1 with "hneg").
+              }
+              iIntros (w).
+              iRewrite -"h1".
+              iSplit; iIntros "#?".
+              { iAssert (interp_type t1 Σthis Σ1 w) with "[hinst]" as "hr"; last by rewrite !interp_type_unfold_v.
+                iApply "hc0".
+                iAssert (go interp_type Σthis Σ0 t1 w) with "[hinst]" as "hh"; last by rewrite !interp_type_unfold_v.
+                by iApply "hinst".
+              }
+              iApply "hinst".
+              iAssert (interp_type t1 Σthis Σ0 w) as "hr"; last by rewrite !interp_type_unfold_v.
+              iApply "hc1".
+              by rewrite !interp_type_unfold_v.
+            * assert (hmono0: mono vs t1).
+              { elim/mono_classI : hmono => cdef' hcdef' hnotcontra hnotcov; simplify_eq.
+                by apply hnotcontra with k Covariant.
+              }
+              iAssert (□ ∀ w, interp_type t1 Σthis Σ0 w -∗ interp_type t1 Σthis Σ1 w)%I as "#hc0".
+              { iDestruct (big_sepL_lookup with "IHty") as "#hk"; first by exact ht1.
+                by iApply ("hk" $! hwf1 Σ0 Σ1 _ _ hmono0 with "h").
+              }
+              iIntros (w).
+              iRewrite -"h1".
+              iIntros "#?".
+              iAssert (interp_type t1 Σthis Σ1 w) with "[hinst]" as "hr"; last by rewrite !interp_type_unfold_v.
+              iApply "hc0".
+              iAssert (go interp_type Σthis Σ0 t1 w) with "[hinst]" as "hh"; last by rewrite !interp_type_unfold_v.
+              by iApply "hinst".
+            * assert (hmono1: mono (neg_variance <$> vs) t1).
+              { elim/mono_classI: hmono => ??? hh; simplify_eq.
+                by apply hh with k Contravariant.
+              }
+              iAssert (□ ∀ w, interp_type t1 Σthis Σ1 w -∗ interp_type t1 Σthis Σ0 w)%I as "#hc1".
+              { iDestruct (big_sepL_lookup with "IHty") as "#hk"; first by exact ht1.
+                by iApply ("hk" $! hwf1 Σ1 Σ0 _ _ hmono1 with "hneg").
+              }
+              iIntros (w).
+              iRewrite -"h1".
+              iIntros "#?".
+              iApply "hinst".
+              iAssert (interp_type t1 Σthis Σ0 w) as "hr"; last by rewrite !interp_type_unfold_v.
+              iApply "hc1".
+              by rewrite !interp_type_unfold_v.
           }
-          assert (hmono1: mono (neg_variance <$> vs) t1).
-          { elim/mono_classI : hmono => cdef' hcdef' hnotcontra hnotcov; simplify_eq.
-            by apply hnotcov with k Invariant.
+          iIntros "htag".
+          iDestruct "htag" as (Σthis0) "(#hcond & #hthism & #htag)".
+          iExists Σthis0; iSplit.
+          { iModIntro; iNext.
+            iIntros (w) "#hthis".
+            iApply "H".
+            by iApply "hcond".
           }
-          iAssert (□ ∀ w, interp_type t1 Σ0 w -∗ interp_type t1 Σ1 w)%I as "#hc0".
-          { iDestruct (big_sepL_lookup with "IHty") as "#hk"; first by exact ht1.
-            by iApply ("hk" $! hwf1 Σ0 Σ1 _ hmono0 with "h").
+          iSplit; first done.
+          iApply "H".
+          by iApply "htag".
+      + iAssert (∀ Σthis0 w0,
+          interp_tag interp_type C Σthis0 (go interp_type Σthis Σ0 <$> σC) w0 -∗
+          interp_tag interp_type C Σthis0 (go interp_type Σthis Σ1 <$> σC) w0)%I as "H".
+          { iIntros (Σthis0 w0) "#htag".
+            rewrite !interp_tag_unseal /interp_tag_def /interp_fun !interp_car_simpl.
+            iDestruct "htag" as (l t cdef tdef σ Σt fields ifields h) "(#hmixed & #hconstr & #hinst & hfields & hloc)".
+            destruct h as (-> & hcdef & htdef & hlΣt & hinherits & hfields & hdom).
+            iExists l, t, cdef, tdef, σ, Σt, fields, ifields.
+            iSplitR; first done.
+            iSplitR.
+            { iModIntro; iNext; iIntros (i ii heq w0) "hii".
+              iSpecialize ("hmixed" $! i ii heq w0 with "hii").
+              iClear "IHty h hinst".
+              iDestruct (interp_mixed_unfold Σthis0 [] w0) as "[hm0 ?]".
+              iDestruct (interp_mixed_unfold Σthis0 [] w0) as "[? hm3]".
+              iDestruct ("hm0" with "hmixed") as "hm".
+              by iApply "hm3".
+            }
+            iSplitR.
+            { iModIntro; iNext; iIntros (i c heq w0) "hc".
+              by iSpecialize ("hconstr" $! i c heq w0 with "hc").
+            }
+            iSplitR; last by iSplit.
+            iModIntro; iNext.
+            iDestruct (iForall3_length with "h") as "%hlen".
+            destruct hlen as [hl0 hl1].
+            iIntros (k var i0 i1 hk) "h0 h1".
+            rewrite !list_lookup_fmap /= !option_equivI /=.
+            destruct (σ !! k) as [t0 | ] eqn:ht0; last done.
+            destruct (σC !! k) as [t1 | ] eqn:ht1; last done.
+            iDestruct (neg_interp_variance with "h") as "hneg".
+            rewrite /= /interp_variance.
+            assert (hwf1: wf_ty t1).
+            { apply wf_tyI in hwf as (? & ? & ? & hwf); simplify_eq.
+              rewrite Forall_lookup in hwf.
+              by apply hwf with k.
+            }
+            iAssert (((λ ty : lang_ty, interp_type ty Σthis0 Σt) <$> σ) !! k ≡ Some (interp_type t0 Σthis0 Σt))%I as "heq0".
+            { by rewrite list_lookup_fmap ht0. }
+            iAssert ((go interp_type Σthis Σ0 <$> σC) !! k ≡ Some (go interp_type Σthis Σ0 t1))%I as "heq1".
+            { by rewrite !list_lookup_fmap /= ht1. }
+            iSpecialize ("hinst" $! k var (interp_type t0 Σthis0 Σt) (go interp_type Σthis Σ0 t1) hk).
+            iSpecialize ("hinst" with "heq0 heq1").
+            destruct var.
+            + assert (hmono0: mono vs t1).
+              { elim/mono_classI: hmono => ?? hh ?; simplify_eq.
+                by apply hh with k Invariant.
+              }
+              assert (hmono1: mono (neg_variance <$> vs) t1).
+              { elim/mono_classI: hmono => ??? hh; simplify_eq.
+                by apply hh with k Invariant.
+              }
+              iAssert (□ ∀ w, interp_type t1 Σthis Σ0 w -∗ interp_type t1 Σthis Σ1 w)%I as "#hc0".
+              { iDestruct (big_sepL_lookup with "IHty") as "#hk"; first by exact ht1.
+                by iApply ("hk" $! hwf1 Σ0 Σ1 _ _ hmono0 with "h").
+              }
+              iAssert (□ ∀ w, interp_type t1 Σthis Σ1 w -∗ interp_type t1 Σthis Σ0 w)%I as "#hc1".
+              { iDestruct (big_sepL_lookup with "IHty") as "#hk"; first by exact ht1.
+                by iApply ("hk" $! hwf1 Σ1 Σ0 _ _ hmono1 with "hneg").
+              }
+              iIntros (w).
+              iRewrite -"h0".
+              iRewrite -"h1".
+              iSplit; iIntros "#?".
+              * iAssert (interp_type t1 Σthis Σ1 w) as "hr"; last by rewrite !interp_type_unfold_v.
+                iApply "hc0".
+                iAssert (go interp_type Σthis Σ0 t1 w) as "hh"; last by rewrite !interp_type_unfold_v.
+                by iApply "hinst".
+              * iApply "hinst".
+                iAssert (interp_type t1 Σthis Σ0 w) as "hr"; last by rewrite !interp_type_unfold_v.
+                iApply "hc1".
+                by rewrite !interp_type_unfold_v.
+            + assert (hmono0: mono vs t1).
+              { elim/mono_classI: hmono => ?? hh ?; simplify_eq.
+                by apply hh with k Covariant.
+              }
+              iAssert (□ ∀ w, interp_type t1 Σthis Σ0 w -∗ interp_type t1 Σthis Σ1 w)%I as "#hc0".
+              { iDestruct (big_sepL_lookup with "IHty") as "#hk"; first by exact ht1.
+                by iApply ("hk" $! hwf1 Σ0 Σ1 _ _ hmono0 with "h").
+              }
+              iIntros (w).
+              iRewrite -"h0".
+              iRewrite -"h1".
+              iIntros "#?".
+              iAssert (interp_type t1 Σthis Σ1 w) as "hr"; last by rewrite !interp_type_unfold_v.
+              iApply "hc0".
+              iAssert (go interp_type Σthis Σ0 t1 w) as "hh"; last by rewrite !interp_type_unfold_v.
+              by iApply "hinst".
+            + assert (hmono1: mono (neg_variance <$> vs) t1).
+              { elim/mono_classI: hmono => ??? hh; simplify_eq.
+                by apply hh with k Contravariant.
+              }
+              iAssert (□ ∀ w, interp_type t1 Σthis Σ1 w -∗ interp_type t1 Σthis Σ0 w)%I as "#hc1".
+              { iDestruct (big_sepL_lookup with "IHty") as "#hk"; first by exact ht1.
+                by iApply ("hk" $! hwf1 Σ1 Σ0 _ _ hmono1 with "hneg").
+              }
+              iIntros (w).
+              iRewrite -"h0".
+              iRewrite -"h1".
+              iIntros "#?".
+              iApply "hinst".
+              iAssert (interp_type t1 Σthis Σ0 w) as "hr"; last by rewrite !interp_type_unfold_v.
+              iApply "hc1".
+              by rewrite !interp_type_unfold_v.
           }
-          iAssert (□ ∀ w, interp_type t1 Σ1 w -∗ interp_type t1 Σ0 w)%I as "#hc1".
-          { iDestruct (big_sepL_lookup with "IHty") as "#hk"; first by exact ht1.
-            by iApply ("hk" $! hwf1 Σ1 Σ0 _ hmono1 with "hneg").
+          iIntros "htag".
+          iDestruct "htag" as (Σthis0) "(#hcond & #hthism & #htag)".
+          iExists Σthis0; iSplit.
+          { iModIntro; iNext.
+            iIntros (w) "#hthis".
+            iApply "H".
+            by iApply "hcond".
           }
-          iIntros (w).
-          iRewrite -"h1".
-          iSplit; iIntros "#?".
-          { iAssert (interp_type t1 Σ1 w) as "hr"; last by rewrite !interp_type_unfold_v.
-            iApply "hc0".
-            iAssert (go interp_type Σ0 t1 w) as "hh"; last by rewrite !interp_type_unfold_v.
-            by iApply "hinst".
-          }
-          iApply "hinst".
-          iAssert (interp_type t1 Σ0 w) as "hr"; last by rewrite !interp_type_unfold_v.
-          iApply "hc1".
-          by rewrite !interp_type_unfold_v.
-        * assert (hmono0: mono vs t1).
-          { elim/mono_classI : hmono => cdef' hcdef' hnotcontra hnotcov; simplify_eq.
-            by apply hnotcontra with k Covariant.
-          }
-          iAssert (□ ∀ w, interp_type t1 Σ0 w -∗ interp_type t1 Σ1 w)%I as "#hc0".
-          { iDestruct (big_sepL_lookup with "IHty") as "#hk"; first by exact ht1.
-            by iApply ("hk" $! hwf1 Σ0 Σ1 _ hmono0 with "h").
-          }
-          iIntros (w).
-          iRewrite -"h1".
-          iIntros "#?".
-          iAssert (interp_type t1 Σ1 w) as "hr"; last by rewrite !interp_type_unfold_v.
-          iApply "hc0".
-          iAssert (go interp_type Σ0 t1 w) as "hh"; last by rewrite !interp_type_unfold_v.
-          by iApply "hinst".
-        * assert (hmono1: mono (neg_variance <$> vs) t1).
-          { elim/mono_classI : hmono => cdef' hcdef' hnotcontra hnotcov; simplify_eq.
-            by apply hnotcov with k Contravariant.
-          }
-          iAssert (□ ∀ w, interp_type t1 Σ1 w -∗ interp_type t1 Σ0 w)%I as "#hc1".
-          { iDestruct (big_sepL_lookup with "IHty") as "#hk"; first by exact ht1.
-            by iApply ("hk" $! hwf1 Σ1 Σ0 _ hmono1 with "hneg").
-          }
-          iIntros (w).
-          iRewrite -"h1".
-          iIntros "#?".
-          iApply "hinst".
-          iAssert (interp_type t1 Σ0 w) as "hr"; last by rewrite !interp_type_unfold_v.
-          iApply "hc1".
-          by rewrite !interp_type_unfold_v.
-      + rewrite !interp_tag_unseal /interp_tag_def /interp_fun !interp_car_simpl.
-        iIntros "htag".
-        iDestruct "htag" as (l t cdef tdef σ Σt fields ifields h) "[#hmixed [#hconstr [#hinst [hdyn hloc]]]]".
-        destruct h as (-> & hcdef & htdef & hlΣt & hinherits & hfields & hdom).
-        iExists l, t, cdef, tdef, σ, Σt, fields, ifields.
-        iSplitR; first done.
-        iSplitR.
-        { iModIntro; iNext; iIntros (i ii heq v) "hii".
-          iSpecialize ("hmixed" $! i ii heq v with "hii").
-          by rewrite !interp_mixed_unfold.
-        }
-        iSplitR.
-        { iModIntro; iNext; iIntros (i c heq v) "hc".
-          by iSpecialize ("hconstr" $! i c heq v with "hc").
-        }
-        iSplitR; last by iSplit.
-        iModIntro; iNext.
-        iDestruct (iForall3_length with "h") as "%hlen".
-        destruct hlen as [hl0 hl1].
-        iIntros (k v i0 i1 hk) "h0 h1".
-        rewrite !list_lookup_fmap.
-        destruct (σ !! k) as [t0 | ] eqn:ht0; last first.
-        { by rewrite !option_equivI. }
-        destruct (σC !! k) as [t1 | ] eqn:ht1; last first.
-        { by rewrite !option_equivI. }
-        rewrite /= !option_equivI.
-        iDestruct (neg_interp_variance with "h") as "hneg".
-        rewrite /interp_variance.
-        assert (hwf1: wf_ty t1).
-        { apply wf_tyI in hwf as (? & ? & ? & hwf); simplify_eq.
-          rewrite Forall_lookup in hwf.
-          by apply hwf with k.
-        }
-        iAssert (Some (interp_type t0 Σt) ≡ Some (interp_type t0 Σt))%I as "heq0"; first done.
-        iAssert (Some (go interp_type Σ0 t1) ≡ Some (go interp_type Σ0 t1))%I as "heq1"; first done.
-        iSpecialize ("hinst" $! k v (interp_type t0 Σt) (go interp_type Σ0 t1) hk).
-        rewrite !list_lookup_fmap /= ht0 ht1.
-        iSpecialize ("hinst" with "heq0 heq1").
-        destruct v.
-        * assert (hmono0: mono vs t1).
-          { elim/mono_classI : hmono => cdef' hcdef' hnotcontra hnotcov; simplify_eq.
-            by apply hnotcontra with k Invariant.
-          }
-          assert (hmono1: mono (neg_variance <$> vs) t1).
-          { elim/mono_classI : hmono => cdef' hcdef' hnotcontra hnotcov; simplify_eq.
-            by apply hnotcov with k Invariant.
-          }
-          iAssert (□ ∀ w, interp_type t1 Σ0 w -∗ interp_type t1 Σ1 w)%I as "#hc0".
-          { iDestruct (big_sepL_lookup with "IHty") as "#hk"; first by exact ht1.
-            by iApply ("hk" $! hwf1 Σ0 Σ1 _ hmono0 with "h").
-          }
-          iAssert (□ ∀ w, interp_type t1 Σ1 w -∗ interp_type t1 Σ0 w)%I as "#hc1".
-          { iDestruct (big_sepL_lookup with "IHty") as "#hk"; first by exact ht1.
-            by iApply ("hk" $! hwf1 Σ1 Σ0 _ hmono1 with "hneg").
-          }
-          iIntros (w).
-          iRewrite -"h0".
-          iRewrite -"h1".
-          iSplit; iIntros "#?".
-          { iAssert (interp_type t1 Σ1 w) as "hr"; last by rewrite !interp_type_unfold_v.
-            iApply "hc0".
-            iAssert (go interp_type Σ0 t1 w) as "hh"; last by rewrite !interp_type_unfold_v.
-            by iApply "hinst".
-          }
-          iApply "hinst".
-          iAssert (interp_type t1 Σ0 w) as "hr"; last by rewrite !interp_type_unfold_v.
-          iApply "hc1".
-          by rewrite !interp_type_unfold_v.
-        * assert (hmono0: mono vs t1).
-          { elim/mono_classI : hmono => cdef' hcdef' hnotcontra hnotcov; simplify_eq.
-            by apply hnotcontra with k Covariant.
-          }
-          iAssert (□ ∀ w, interp_type t1 Σ0 w -∗ interp_type t1 Σ1 w)%I as "#hc0".
-          { iDestruct (big_sepL_lookup with "IHty") as "#hk"; first by exact ht1.
-            by iApply ("hk" $! hwf1 Σ0 Σ1 _ hmono0 with "h").
-          }
-          iIntros (w).
-          iRewrite -"h0".
-          iRewrite -"h1".
-          iIntros "#?".
-          iAssert (interp_type t1 Σ1 w) as "hr"; last by rewrite !interp_type_unfold_v.
-          iApply "hc0".
-          iAssert (go interp_type Σ0 t1 w) as "hh"; last by rewrite !interp_type_unfold_v.
-          by iApply "hinst".
-        * assert (hmono1: mono (neg_variance <$> vs) t1).
-          { elim/mono_classI : hmono => cdef' hcdef' hnotcontra hnotcov; simplify_eq.
-            by apply hnotcov with k Contravariant.
-          }
-          iAssert (□ ∀ w, interp_type t1 Σ1 w -∗ interp_type t1 Σ0 w)%I as "#hc1".
-          { iDestruct (big_sepL_lookup with "IHty") as "#hk"; first by exact ht1.
-            by iApply ("hk" $! hwf1 Σ1 Σ0 _ hmono1 with "hneg").
-          }
-          iIntros (w).
-          iRewrite -"h0".
-          iRewrite -"h1".
-          iIntros "#?".
-          iApply "hinst".
-          iAssert (interp_type t1 Σ0 w) as "hr"; last by rewrite !interp_type_unfold_v.
-          iApply "hc1".
-          by rewrite !interp_type_unfold_v.
+          iSplit; first done.
+          iApply "H".
+          by iApply "htag".
+    - by iIntros "hh".
     - iIntros "hh".
       iDestruct "hh" as "[hint | hh]"; first by iLeft.
       iDestruct "hh" as "[hbool | hh]"; first by (iRight; iLeft).
@@ -1590,11 +2219,13 @@ Section proofs.
       { destruct (Σ0 !! i) as [ ? | ] eqn:h0.
         { apply lookup_ge_None_1 in hvi.
           apply lookup_lt_Some in h0.
+          simpl in *.
           by lia.
         }
         destruct (Σ1 !! i) as [ ? | ] eqn:h1.
         { apply lookup_ge_None_1 in hvi.
           apply lookup_lt_Some in h1.
+          simpl in *.
           by lia.
         }
         by rewrite /interp_generic h0 h1.
@@ -1602,11 +2233,13 @@ Section proofs.
       destruct (Σ0 !! i) as [ i0 | ] eqn:h0; last first.
       { apply lookup_ge_None_1 in h0.
         apply lookup_lt_Some in hvi.
+        simpl in *.
         by lia.
       }
       destruct (Σ1 !! i) as [ i1 | ] eqn:h1; last first.
       { apply lookup_ge_None_1 in h1.
         apply lookup_lt_Some in hvi.
+        simpl in *.
         by lia.
       }
       simpl.
@@ -1621,12 +2254,13 @@ Section proofs.
       * by iSpecialize ("hf" $! v).
     - by iIntros "hh".
     - by iIntros "hh".
+    - by iIntros "hh".
   Qed.
 
   Lemma interp_env_with_mono :
     map_Forall (λ _ : string, wf_cdef_mono) pdefs →
     map_Forall (λ _ : string, wf_cdef_parent pdefs) pdefs →
-    ∀ σ vs Σ0 Σ1 ws,
+    ∀ σ vs (Σthis : interp Θ) (Σ0 Σ1: list (interp Θ)) ws,
     Forall wf_ty σ →
     length σ = length ws →
     (∀ i wi ti, ws !! i = Some wi →
@@ -1638,10 +2272,11 @@ Section proofs.
                 not_cov wi →
                 mono (neg_variance <$> vs) ti) →
     □ iForall3 interp_variance vs Σ0 Σ1 -∗
-    iForall3 interp_variance ws (interp_list Σ0 σ) (interp_list Σ1 σ).
+    iForall3 interp_variance ws
+      (interp_list Σthis Σ0 σ) (interp_list Σthis Σ1 σ).
   Proof.
     move => hmono hp.
-    induction σ as [ | ty σ hi] => //= vs Σ0 Σ1 ws hwf hlen hcov hcontra.
+    induction σ as [ | ty σ hi] => //= vs Σthis Σ0 Σ1 ws hwf hlen hcov hcontra.
     { rewrite (nil_length_inv ws) //.
       by iIntros.
     }
@@ -1673,24 +2308,23 @@ Section proofs.
     map_Forall (λ _cname, wf_cdef_parent pdefs) pdefs →
     map_Forall (λ _ : string, wf_cdef_mono) pdefs →
     ∀ A B σB, extends_using A B σB →
-    ∀ Σ v,
-    interp_tag_alt Σ A v -∗
-    interp_tag_alt (interp_list Σ σB) B v.
+    ∀ Σthis Σ v, interp_tag_alt A Σthis Σ v -∗
+    interp_tag_alt B Σthis (interp_list Σthis Σ σB) v.
   Proof.
-    move => hwp hmono A B σB hext Σ v.
-    assert (hb: ∃ bdef, pdefs !! B = Some bdef ∧ length bdef.(generics) = length (interp_list Σ σB)).
+    move => hwp hmono A B σB hext Σthis Σ v.
+    iIntros "#h".
+    iDestruct "h" as (ℓ t adef tdef σ Σt fields ifields) "(%h & #hmixed & #hconstr & #hinst & hdyn & hl)".
+    destruct h as (-> & hadef & htdef & hlΣt & hin & hfields & hdom); simplify_eq.
+    assert (hb: ∃ bdef, pdefs !! B = Some bdef ∧ length bdef.(generics) = length (interp_list Σthis Σ σB)).
     { apply extends_using_wf in hext => //.
-      destruct hext as (? & ? & ? & h).
+      destruct hext as (? & ? & ? & h & _).
       apply wf_tyI in h as (bdef & ? & ? & ?); simplify_eq.
       exists bdef; repeat split => //.
       by rewrite /interp_list fmap_length.
     }
     destruct hb as (bdef & hbdef & hlen2).
-    iIntros "h".
-    iDestruct "h" as (ℓ t adef tdef σ Σt fields ifields) "(%h & #hmixed & #hconstr & #hinst & hdyn & hl)".
-    destruct h as (-> & hadef & htdef & hlΣt & hin & hfields & hdom); simplify_eq.
-    destruct (extends_using_wf _ _ _ hwp hext) as (adef' & hadef' & hF & hwfB).
-    destruct (inherits_using_wf _ _ _ hwp hin) as (tdef' & htdef' & htF & hwfA).
+    destruct (extends_using_wf _ _ _ hwp hext) as (adef' & hadef' & hF & hwfB & _).
+    destruct (inherits_using_wf _ _ _ hwp hin) as (tdef' & htdef' & htF & hwfA & _).
     simplify_eq.
     iExists ℓ, t, bdef, tdef, (subst_ty σ <$> σB), Σt, fields, ifields.
     iSplit.
@@ -1701,8 +2335,8 @@ Section proofs.
     iSplitR => //.
     iSplitR; last by iSplit.
     iModIntro; iNext.
-    assert (heq: interp_list Σt (subst_ty σ <$> σB) ≡ interp_list (interp_list Σt σ) σB).
-    { rewrite /interp_list -!list_fmap_compose.
+    assert (heq: interp_list Σthis Σt (subst_ty σ <$> σB) ≡ interp_list Σthis (interp_list Σthis Σt σ) σB).
+    { rewrite /interp_list -!list_fmap_compose /=.
       apply list_fmap_equiv_ext => ? ty0 hin0 /= w.
       apply elem_of_list_lookup_2 in hin0.
       rewrite interp_type_subst //.
@@ -1711,8 +2345,8 @@ Section proofs.
       rewrite hlen.
       by apply hF.
     }
-    rewrite (iForall3_interp_equivI_l _ _ heq bdef.(generics) (interp_list Σ σB)).
-    iApply (interp_env_with_mono with "hinst") => //.
+    rewrite (iForall3_interp_equivI_l _ _ heq bdef.(generics) (interp_list Σthis Σ σB)) => {heq}.
+    iApply (interp_env_with_mono hmono hwp _ _ Σthis with "hinst").
     + by apply wf_ty_classI in hwfB.
     + apply wf_tyI in hwfB as [? [? [??]]]; by simplify_eq.
     + move => i wi ti hwi hti hc.
@@ -1723,29 +2357,65 @@ Section proofs.
       elim/mono_classI : hext => bdef' hbdef' ??; simplify_eq; by eauto.
   Qed.
 
+  (* σb doesn't have `this` so we don't care which Σthis is used for it *)
+  Lemma class_extends_using_is_inclusion:
+    map_Forall (λ _cname, wf_cdef_parent pdefs) pdefs →
+    map_Forall (λ _ : string, wf_cdef_mono) pdefs →
+    ∀ A B σB, extends_using A B σB →
+    ∀ Σthis Σ v, interp_class_alt A Σ v -∗
+    interp_class_alt B (interp_list Σthis Σ σB) v.
+  Proof.
+    move => hwp hmono A B σB hext Σthis Σ v.
+    iIntros "#h".
+    iDestruct "h" as (Σthis0) "(#hcond & #thism & #htag)".
+    iExists Σthis0.
+    iAssert (∀ Σthis0 v, interp_tag_alt A Σthis0 Σ v -∗
+             interp_tag_alt B Σthis0 (interp_list Σthis Σ σB) v)%I as "h".
+    { iIntros (Σthis1 ?) "#h".
+      iDestruct (tag_extends_using_is_inclusion with "h") as "hh" => //.
+      apply extends_using_wf in hext => //.
+      destruct hext as (adef & hadef & _ & hwfB & hnothis).
+      apply wf_tyI in hwfB as (? & ? & ? & ?).
+      iApply (interp_tag_alt_equivI Σthis1); last done.
+      + done.
+      + by apply interp_list_no_this.
+      + done.
+      + by rewrite /interp_list fmap_length.
+    }
+    iSplit.
+    - iModIntro; iNext.
+      iIntros (w) "#hthis".
+      iSpecialize ("hcond" with "hthis").
+      by iApply "h".
+    - iSplit; first done.
+      by iApply "h".
+  Qed.
+
   (* if class A<..> extends B<σB>, then for any valid substitution σA,
    * [| A<σA> |] ⊆ [| B<σA o σB> |]
    *)
   Lemma extends_using_is_inclusion:
     map_Forall (λ _cname, wf_cdef_parent pdefs) pdefs →
     map_Forall (λ _ : string, wf_cdef_mono) pdefs →
-    ∀ Σ A B σA σB v, extends_using A B σB →
+    ∀ Σthis Σ A B σA σB v, extends_using A B σB →
     wf_ty (ClassT true A σA) →
-    interp_type (ClassT false A σA) Σ v -∗
-    interp_type (ClassT false B (subst_ty σA <$> σB)) Σ v.
+    interp_type (ClassT false A σA) Σthis Σ v -∗
+    interp_type (ClassT false B (subst_ty σA <$> σB)) Σthis Σ v.
   Proof.
-    move => hp ? Σ A B σA σB v hext hwfA.
+    move => hp hmono Σthis Σ A B σA σB v hext hwfA.
+    rewrite interp_class_unfold //.
     iIntros "h".
     assert (hb: wf_ty (ClassT true B σB)).
     { apply extends_using_wf in hext => //.
-      by destruct hext as (?&?&?&?).
+      by repeat destruct hext as [? hext].
     }
     assert (hb0 := hb).
     apply wf_tyI in hb0 as [? [? [??]]].
     rewrite !interp_class_unfold //.
-    - iDestruct (tag_extends_using_is_inclusion with "h") as "hh" => //.
-      assert (hΣ : interp_list Σ (subst_ty σA <$> σB) ≡
-                   interp_list (interp_list Σ σA) σB).
+    - iDestruct (class_extends_using_is_inclusion with "h") as "hh";
+       [ done | done | exact hext | ].
+      assert (hΣ : interp_list Σthis Σ (subst_ty σA <$> σB) ≡
+                   interp_list Σthis (interp_list Σthis Σ σA) σB).
       { rewrite /interp_list -list_fmap_compose.
         apply list_fmap_equiv_ext  => ? ty0 hin0 /= w.
         apply elem_of_list_lookup_2 in hin0.
@@ -1757,7 +2427,7 @@ Section proofs.
         rewrite hlen; by apply hF.
       }
       assert (h0 := hwfA); apply wf_tyI in hwfA as (? & ? & ? & ?).
-      rewrite (interp_tag_alt_equivI _ _ hp hΣ) //.
+      rewrite (interp_class_alt_equivI _ _ hp hΣ) //.
       by rewrite /interp_list !map_length.
     - change (wf_ty (ClassT true B (subst_ty σA <$> σB))) with (wf_ty (subst_ty σA (ClassT true B σB))).
       apply wf_ty_subst => //.
@@ -1767,12 +2437,12 @@ Section proofs.
   Lemma inherits_using_is_inclusion:
     map_Forall (λ _cname, wf_cdef_parent pdefs) pdefs →
     map_Forall (λ _ : string, wf_cdef_mono) pdefs →
-    ∀ Σ A B σA σB v, inherits_using A B σB →
+    ∀ Σthis Σ A B σA σB v, inherits_using A B σB →
     wf_ty (ClassT true A σA) →
-    interp_type (ClassT false A σA) Σ v -∗
-    interp_type (ClassT false B (subst_ty σA <$> σB)) Σ v.
+    interp_type (ClassT false A σA) Σthis Σ v -∗
+    interp_type (ClassT false B (subst_ty σA <$> σB)) Σthis Σ v.
   Proof.
-    move => ?? Σ A B σA σB v h.
+    move => ?? Σthis Σ A B σA σB v h.
     move : σA v.
     induction h as [ A adef hpdefs | A B σ hext | A B σ C σC hext h hi ]
         => σA v hwf.
@@ -1783,12 +2453,12 @@ Section proofs.
     - iIntros "h".
       iDestruct (extends_using_is_inclusion with "h") as "he" => //.
       apply extends_using_wf in hext => //.
-      destruct hext as (? & ? & ? & hwfB).
+      destruct hext as (? & ? & ? & hwfB & _).
       rewrite map_subst_ty_subst; last first.
       { apply inherits_using_wf in h => //.
-        destruct h as (bdef & hbdef & hb & hwfC).
+        destruct h as (bdef & hbdef & hb & hwfC & _).
         replace (length σ) with (length bdef.(generics)); first done.
-        inv hwfB; by simplify_eq.
+        apply wf_tyI in hwfB as (? & ? & ? & ?); by simplify_eq.
       }
       iApply hi => //.
       assert (h_ := hwfB).
@@ -1805,17 +2475,18 @@ Section proofs.
     Hypothesis wf_parent : map_Forall (λ _cname, wf_cdef_parent pdefs) pdefs.
     Hypothesis wf_mono : map_Forall (λ _ : string, wf_cdef_mono) pdefs.
     Hypothesis wf_constraints_wf : map_Forall (λ _cname, wf_cdef_constraints_wf) pdefs.
+    Hypothesis wf_constraints_no_this : map_Forall (λ _cname, wf_cdef_constraints_no_this) pdefs.
     Hypothesis wf_constraints_bounded : map_Forall (λ _cname, wf_cdef_constraints_bounded) pdefs.
 
   (* Extracting subproofs for clarity *)
-  Lemma subvariance_is_inclusion_aux Σ:
+  Lemma subvariance_is_inclusion_aux Σthis Σ:
     ∀ exact_ A adef σ0 σ1 v,
     pdefs !! A = Some adef →
     wf_ty (ClassT true A σ0) →
     Forall wf_ty σ1 →
-    ⊢ □ iForall3 interp_variance adef.(generics) (interp_list Σ σ0) (interp_list Σ σ1) →
-    interp_type (ClassT exact_ A σ0) Σ v -∗
-    interp_type (ClassT exact_ A σ1) Σ v.
+    ⊢ □ iForall3 interp_variance adef.(generics) (interp_list Σthis Σ σ0) (interp_list Σthis Σ σ1) →
+    interp_type (ClassT exact_ A σ0) Σthis Σ v -∗
+    interp_type (ClassT exact_ A σ1) Σthis Σ v.
   Proof.
     move => exact_ A adef σ0 σ1 v hadef hwfA hwfσ1.
     iIntros "#hσ #h".
@@ -1826,41 +2497,65 @@ Section proofs.
       by destruct hh.
     }
     case: exact_.
-    - rewrite !interp_class_unfold_exact //; last first.
+    - rewrite !interp_exact_class_unfold //; last first.
       { econstructor => //.
         apply wf_tyI in hwfA as (? & ? & ? & ?); simplify_eq.
         by rewrite -hl0.
       }
-      iDestruct "h" as (l adef' Σa fields ifields h) "(#hmixed & #hconstr & #hinst & hdyn & hl)".
-      destruct h as (-> & hadef' & hlΣa & hfields & hdom); simplify_eq.
-      iExists l, adef, Σa, fields, ifields.
+      iAssert (∀ Σthis0 v,
+        interp_exact_tag_alt A Σthis0 (interp_list Σthis Σ σ0) v -∗
+        interp_exact_tag_alt A Σthis0 (interp_list Σthis Σ σ1) v)%I as "htag".
+      { iIntros (Σthis0 ?) "htag".
+        iDestruct "htag" as (l adef' Σa fields ifields h) "(#hmixed & #hconstr & #hinst & hfields & hl)".
+        destruct h as (-> & hadef' & hlΣa & hfields & hdom); simplify_eq.
+        iExists l, adef, Σa, fields, ifields.
+        iSplit; first done.
+        iSplit; first done.
+        iSplit; first done.
+        iSplit; last by iSplit.
+        iModIntro; iNext.
+        by iApply (iForall3_interp_trans with "hinst hσ").
+      }
+      iDestruct "h" as (Σthis0) "(#hcond & #hmixed0 & #h)".
+      iExists Σthis0; iSplit.
+      { iModIntro; iNext; iIntros (w) "#hthis".
+        iApply "htag".
+        by iApply "hcond".
+      }
       iSplit; first done.
-      iSplit; first done.
-      iSplit; first done.
-      iSplit; last by iSplit.
-      iModIntro; iNext.
-      iClear "hdyn hl hmixed".
-      by iApply (iForall3_interp_trans with "hinst hσ").
+      by iApply "htag".
     - rewrite !interp_class_unfold //; last first.
       { econstructor => //.
         apply wf_tyI in hwfA as (? & ? & ? & ?); simplify_eq.
         by rewrite -hl0.
       }
-      iDestruct "h" as (l t adef' tdef σ Σt fields ifields h) "(#hmixed & #hconstr & #hinst & hdyn & hl)".
-      destruct h as (-> & hadef' & tdef' & hlΣa & hin &  hfields & hdom); simplify_eq.
-      iExists l, t, adef, tdef, σ, Σt, fields, ifields.
+      iAssert (∀ Σthis0 v,
+        interp_tag_alt A Σthis0 (interp_list Σthis Σ σ0) v -∗
+        interp_tag_alt A Σthis0 (interp_list Σthis Σ σ1) v)%I as "htag".
+      { iIntros (Σthis0 ?) "htag".
+        iDestruct "htag" as (l t adef' tdef σ Σt fields ifields h) "(#hmixed & #hconstr & #hinst & hfields & hl)".
+        destruct h as (-> & hadef' & tdef' & hlΣa & hin &  hfields & hdom); simplify_eq.
+        iExists l, t, adef, tdef, σ, Σt, fields, ifields.
+        iSplit; first done.
+        iSplit; first done.
+        iSplit; first done.
+        iSplit; last by iSplit.
+        iModIntro; iNext.
+        by iApply (iForall3_interp_trans with "hinst hσ").
+      }
+      iDestruct "h" as (Σthis0) "(#hcond & #hmixed0 & #h)".
+      iExists Σthis0; iSplit.
+      { iModIntro; iNext; iIntros (w) "#hthis".
+        iApply "htag".
+        by iApply "hcond".
+      }
       iSplit; first done.
-      iSplit; first done.
-      iSplit; first done.
-      iSplit; last by iSplit.
-      iModIntro; iNext.
-      iClear "hdyn hl hmixed".
-      by iApply (iForall3_interp_trans with "hinst hσ").
+      by iApply "htag".
   Qed.
 
-  Lemma exact_subtype_is_inclusion_aux Σ A v:
-    interp_exact_tag interp_type Σ A v -∗
-    interp_tag interp_type Σ A v.
+  Lemma exact_subtype_is_inclusion_aux Σthis Σ A v:
+    interp_exact_tag interp_type A Σthis Σ v -∗
+    interp_tag interp_type A Σthis Σ v.
   Proof.
     rewrite interp_tag_unseal /interp_tag_def.
     rewrite interp_exact_tag_unseal /interp_exact_tag_def /=.
@@ -1891,35 +2586,50 @@ Section proofs.
     by iApply ("hinst" $! k v i0 i1 hk with "ha h1").
   Qed.
 
-  Lemma exact_subtype_is_inclusion Σ exact_ A σ v:
-    interp_type (ClassT exact_ A σ) Σ v -∗
-    interp_type (ClassT false A σ) Σ v.
+  Lemma exact_class_subtype_is_inclusion Σ A v:
+    interp_exact_class interp_type A Σ v -∗
+    interp_class interp_type A Σ v.
+  Proof.
+    iIntros "h".
+    iDestruct "h" as (Σthis0) "(#hcond & #hmixed & #h)".
+    iExists Σthis0; iSplit.
+    { iModIntro; iNext; iIntros (w) "hh".
+      iApply exact_subtype_is_inclusion_aux.
+      by iApply "hcond".
+    }
+    iSplit; first done.
+    by iApply exact_subtype_is_inclusion_aux.
+  Qed.
+
+  Lemma exact_subtype_is_inclusion Σthis Σ exact_ A σ v:
+    interp_type (ClassT exact_ A σ) Σthis Σ v -∗
+    interp_type (ClassT false A σ) Σthis Σ v.
   Proof.
     destruct exact_; last done.
     rewrite interp_type_unfold /=.
     rewrite interp_type_unfold /=.
     iIntros "h".
-    by iApply exact_subtype_is_inclusion_aux.
+    by iApply exact_class_subtype_is_inclusion.
   Qed.
 
-  Lemma submixed_is_inclusion_aux Σ:
+  Lemma submixed_is_inclusion_aux Σthis Σ:
     ∀ A v, wf_ty A →
+    □ interp_as_mixed Σthis -∗
     □ interp_env_as_mixed Σ -∗
-    interp_type A Σ v -∗
-    interp_type MixedT Σ v.
+    interp_type A Σthis Σ v -∗
+    interp_type MixedT Σthis Σ v.
   Proof.
-    iIntros (A v hwf) "#wfΣi h".
+    iIntros (A v hwf) "#wfThis #wfΣ h".
     rewrite !interp_type_unfold /=.
-    iInduction A as [ | | | | exact_ C σC hi | | | A B hA hB | A B hA hB | i | | ]
+    iInduction A as [ | | | | exact_ C σC hi | | | A B hA hB | A B hA hB | i | | | ]
         "IHty" forall (v hwf).
     - by repeat iLeft.
     - by iLeft; iRight; iLeft.
     - done.
     - done.
     - iLeft; iRight; iRight => /=.
-      iExists C.
-      iExists (interp_list Σ σC).
-      assert (heq: (go interp_type Σ <$> σC) ≡ interp_list Σ σC).
+      iExists C, (interp_list Σthis Σ σC).
+      assert (heq: go interp_type Σthis Σ <$> σC ≡ interp_list Σthis Σ σC).
       { rewrite /interp_list.
         apply list_fmap_equiv_ext => ? ty ? w.
         by rewrite interp_type_unfold.
@@ -1927,9 +2637,25 @@ Section proofs.
       apply wf_tyI in hwf as (cdef & ? & ? & ?).
       iExists cdef; iSplit.
       { by rewrite /interp_list map_length. }
-      rewrite -(interp_tag_equivI _ _ heq C v).
-      destruct exact_; last done.
-      by iApply exact_subtype_is_inclusion_aux.
+      destruct exact_.
+      + iDestruct "h" as (Σthis0) "(#hcond & #hmxied & #h)".
+        iExists Σthis0; iSplit.
+        { iModIntro; iNext; iIntros (w) "#hthis".
+          iApply exact_subtype_is_inclusion_aux.
+          rewrite -(interp_exact_tag_equivI _ _ _ heq C w).
+          by iApply "hcond".
+        }
+        iSplit; first done.
+        iApply exact_subtype_is_inclusion_aux.
+        by rewrite -(interp_exact_tag_equivI _ _ _ heq C v).
+      + iDestruct "h" as (Σthis0) "(#hcond & #hmxied & #h)".
+        iExists Σthis0; iSplit.
+        { iModIntro; iNext; iIntros (w) "#hthis".
+          rewrite -(interp_tag_equivI _ _ _ heq C w).
+          by iApply "hcond".
+        }
+        iSplit; first done.
+        by rewrite -(interp_tag_equivI _ _ _ heq C v).
     - by iRight.
     - by iLeft.
     - apply wf_tyI in hwf as [??].
@@ -1940,10 +2666,9 @@ Section proofs.
     - rewrite /= /interp_generic.
       destruct (decide (i < length Σ)) as [hlt | hge].
       + apply lookup_lt_is_Some_2 in hlt as [ϕ hϕ].
-        iApply "wfΣi"; last done.
-        by rewrite /= /interp_generic hϕ /=.
-      + rewrite /= /interp_generic lookup_ge_None_2 /=; last by apply not_lt.
-        done.
+        iApply ("wfΣ" $! i); last done.
+        by rewrite hϕ /=.
+      + by rewrite /= /interp_generic lookup_ge_None_2 /=; last by apply not_lt.
     - rewrite /= /interp_dynamic.
       iDestruct "h" as "[? | h]".
       { by iLeft; iLeft. }
@@ -1952,8 +2677,12 @@ Section proofs.
       iDestruct "h" as "[? | h]".
       { by iRight. }
       iLeft; iRight; iRight.
-      iDestruct "h" as (t Σt def [h0 h1]) "(? & ? & ? & ?)".
-      iExists t, Σt, def; by iSplit.
+      iDestruct "h" as (t Σthis0 Σt def [h0 h1]) "(? & ? & ? & ? & ? & ?)".
+      iExists t, Σt, def.
+      iSplit; first done.
+      iExists Σthis0.
+      iSplit; first done.
+      by iSplit.
     - iDestruct "h" as "[hz | h]".
       { iLeft; by iLeft. }
       iDestruct "h" as "[hb | h]".
@@ -1961,33 +2690,38 @@ Section proofs.
       iDestruct "h" as "[hn | h]".
       { by iRight. }
       iLeft; iRight; iRight.
-      iDestruct "h" as (t Σt def h) "(? & ? & ? & ?)".
-      by iExists _, _, _; iSplit.
+      iDestruct "h" as (t Σt def h) "(? & ? & ? & ? & ? & ? & ?)".
+      iExists _, _, _; iSplit; first done.
+      iExists _; iSplit; first done.
+      by iSplit.
+    - by iSpecialize ("wfThis" $! v with "h").
   Qed.
 
   (* Main meat for A <: B → [|A|] ⊆ [|B|] *)
-  Theorem subtype_is_inclusion_aux kd Σ A B:
+  Theorem subtype_is_inclusion_aux kd Σthis Σ A B:
     subtype Δ kd A B →
     ∀ v,
     wf_ty A →
+    □ interp_as_mixed Σthis -∗
     □ interp_env_as_mixed Σ -∗
-    □ Σinterp Σ Δ -∗
-    interp_type_pre interp_type A Σ v -∗
-    interp_type_pre interp_type B Σ v
-    with subtype_targs_is_inclusion_aux kd Σ Vs As Bs:
+    □ Σinterp Σthis Σ Δ -∗
+    interp_type_pre interp_type A Σthis Σ v -∗
+    interp_type_pre interp_type B Σthis Σ v
+    with subtype_targs_is_inclusion_aux kd Σthis Σ Vs As Bs:
     Forall wf_ty As →
     Forall wf_ty Bs →
     subtype_targs Δ kd Vs As Bs →
+    □ interp_as_mixed Σthis -∗
     □ interp_env_as_mixed Σ -∗
-    □ Σinterp Σ Δ -∗
-    □ iForall3 interp_variance Vs (interp_list Σ As) (interp_list Σ Bs).
+    □ Σinterp Σthis Σ Δ -∗
+    □ iForall3 interp_variance Vs (interp_list Σthis Σ As) (interp_list Σthis Σ Bs).
   Proof.
     { destruct 1 as [ kd A | kd A h | kd A σA B σB adef hadef hlen hext
       | kd A σA adef hadef hlen
-      | kd ? A def σ0 σ1 hadef hwfσ hσ | | | | | | kd A B h
+      | kd exact_ A def σ0 σ1 hadef hwfσ hσ | | | | | kd exact_ ?? | kd A B h
       | kd A B h | kd A B C h0 h1 | kd A B | kd A B | kd A B C h0 h1
-      | | kd A B C h0 h1 | kd A B hin | kd ? A adef σA hadef _ hf0 hf1
-      | | | | | | kd A B hwf h ]; iIntros (v hwfA) "#wfΣ #Σcoherency #h".
+      | | kd A B C h0 h1 | kd A B hin | kd exact_ A adef σA hadef _ hf0 hf1
+      | | | | | | kd A B hwf h ]; iIntros (v hwfA) "#wfThis #wfΣ #Σcoherency #h".
       - clear subtype_is_inclusion_aux subtype_targs_is_inclusion_aux.
         rewrite -!interp_type_unfold.
         by iApply submixed_is_inclusion_aux.
@@ -1998,8 +2732,8 @@ Section proofs.
         { apply wf_tyI in hwfA as (? & ? & ?& ?); simplify_eq; by econstructor. }
         rewrite -!interp_type_unfold; by iApply extends_using_is_inclusion.
       - clear subtype_targs_is_inclusion_aux subtype_is_inclusion_aux.
-        by iApply exact_subtype_is_inclusion_aux.
-      - apply subtype_targs_is_inclusion_aux with (Σ := Σ) in hσ => //; last first.
+        by iApply exact_class_subtype_is_inclusion.
+      - apply subtype_targs_is_inclusion_aux with (Σthis := Σthis) (Σ := Σ) in hσ => //; last first.
         { by apply wf_ty_classI in hwfA. }
         clear subtype_is_inclusion_aux subtype_targs_is_inclusion_aux.
         rewrite -!interp_type_unfold.
@@ -2022,10 +2756,18 @@ Section proofs.
         iRight; iRight.
         assert (h0 := hwfA).
         apply wf_tyI in h0 as (adef & ? & ?& ?); simplify_eq.
-        iExists A, (go interp_type Σ <$> targs), adef; iSplit.
+        iExists A, (interp_list Σthis Σ targs), adef; iSplit.
         { by rewrite map_length. }
-        destruct exact; last done.
-        by iApply exact_subtype_is_inclusion_aux.
+        destruct exact_.
+        + iApply exact_class_subtype_is_inclusion.
+          rewrite -interp_type_unfold.
+          rewrite interp_exact_class_unfold //.
+          rewrite interp_exact_class_equiv //.
+          by rewrite /interp_list fmap_length.
+        + rewrite -interp_type_unfold.
+          rewrite interp_class_unfold //; last by eapply wf_ty_exact.
+          rewrite interp_class_equiv //.
+          by rewrite /interp_list fmap_length.
       - clear subtype_is_inclusion_aux subtype_targs_is_inclusion_aux.
         by iLeft.
       - clear subtype_is_inclusion_aux subtype_targs_is_inclusion_aux.
@@ -2033,10 +2775,10 @@ Section proofs.
       - clear subtype_targs_is_inclusion_aux.
         rewrite /= /interp_union.
         iDestruct "h" as "[h | h]".
-        + iApply (subtype_is_inclusion_aux with "wfΣ Σcoherency"); [exact h0 | | ].
+        + iApply (subtype_is_inclusion_aux with "wfThis wfΣ Σcoherency"); [exact h0 | | ].
           * apply wf_tyI in hwfA as [??]; by assumption.
           * by iAssumption.
-        + iApply (subtype_is_inclusion_aux with "wfΣ Σcoherency"); [exact h1 | | ].
+        + iApply (subtype_is_inclusion_aux with "wfThis wfΣ Σcoherency"); [exact h1 | | ].
           * apply wf_tyI in hwfA as [??]; by assumption.
           * by iAssumption.
       - clear subtype_is_inclusion_aux subtype_targs_is_inclusion_aux.
@@ -2048,15 +2790,15 @@ Section proofs.
       - clear subtype_targs_is_inclusion_aux.
         rewrite /= /interp_inter.
         iSplit.
-        + iApply (subtype_is_inclusion_aux with "wfΣ Σcoherency"); [exact h0 | done | ].
+        + iApply (subtype_is_inclusion_aux with "wfThis wfΣ Σcoherency"); [exact h0 | done | ].
           by iAssumption.
-        + iApply (subtype_is_inclusion_aux with "wfΣ Σcoherency"); [exact h1 | done | ].
+        + iApply (subtype_is_inclusion_aux with "wfThis wfΣ Σcoherency"); [exact h1 | done | ].
           by iAssumption.
       - done.
-      - iApply (subtype_is_inclusion_aux with "wfΣ Σcoherency"); [exact h1 | | ].
+      - iApply (subtype_is_inclusion_aux with "wfThis wfΣ Σcoherency"); [exact h1 | | ].
         + apply subtype_wf in h0; [ | done | done | done ].
           by assumption.
-        + iApply (subtype_is_inclusion_aux with "wfΣ Σcoherency"); [exact h0 | done | ].
+        + iApply (subtype_is_inclusion_aux with "wfThis wfΣ Σcoherency"); [exact h0 | done | ].
           by iAssumption.
       - apply elem_of_list_lookup_1 in hin as [i hin].
         rewrite -!interp_type_unfold /=.
@@ -2064,7 +2806,14 @@ Section proofs.
       - iRight; iRight; iRight.
         assert (hl : length σA = length adef.(generics)).
         { apply wf_tyI in hwfA as (? & ? & ?& ?); by simplify_eq. }
-        iExists A, (interp_list Σ σA), adef; iSplit.
+        simpl.
+        iAssert (interp_class interp_type A (go interp_type Σthis Σ <$> σA) v) as "hsimpl".
+        { destruct exact_; last done.
+          by iApply exact_class_subtype_is_inclusion.
+        }
+        iClear "h".
+        iDestruct "hsimpl" as (Σthis0) "(#hcond & #hthism & #htag)".
+        iExists A, Σthis0, (interp_list Σthis Σ σA), adef; iSplit.
         { by rewrite /interp_list map_length. }
         iSplit; first last.
         + iSplit; last iSplit.
@@ -2075,9 +2824,9 @@ Section proofs.
               rewrite Forall_lookup in hwf.
               by eauto.
             }
-            rewrite (interp_type_unfold [] MixedT w).
-            rewrite -(interp_type_unfold Σ MixedT w).
-            by iApply (submixed_is_inclusion_aux Σ).
+            rewrite (interp_type_unfold Σthis0 [] MixedT w).
+            rewrite -(interp_type_unfold Σthis Σ MixedT w).
+            by iApply (submixed_is_inclusion_aux Σthis Σ).
           * iModIntro; iNext; iIntros (i [s t] hc w) "#h1".
             assert (hwf: wf_ty (subst_ty σA s)).
             { apply wf_ty_subst => //; first by apply wf_ty_classI in hwfA.
@@ -2092,18 +2841,30 @@ Section proofs.
               by rewrite hl.
             }
             destruct hb as [].
+            assert (hno: no_this_constraint (s, t)).
+            { apply wf_constraints_no_this in hadef.
+              rewrite /wf_cdef_constraints_no_this Forall_lookup in hadef.
+              by apply hadef in hc.
+            }
+            destruct hno as [].
             apply hf1 in hc; simpl in *.
+            rewrite (interp_type_no_this _ _ _ Σthis0 Σthis) //.
+            rewrite (interp_type_no_this _ _ _ Σthis0 Σthis) //.
             rewrite -!interp_type_subst //.
-            rewrite !interp_type_unfold.
+            rewrite !interp_type_unfold_v.
             by iApply subtype_is_inclusion_aux.
-          * assert (heq: interp_list Σ σA ≡ go interp_type Σ <$> σA).
+          * assert (heq: interp_list Σthis Σ σA ≡ go interp_type Σthis Σ <$> σA).
             { rewrite /interp_list.
               apply list_fmap_equiv_ext => ? ty hty w.
               by rewrite interp_type_unfold.
             }
-            rewrite (interp_tag_equivI _ _ heq).
-            destruct exact; last done.
-            by iApply exact_subtype_is_inclusion_aux.
+            iSplit.
+            { iModIntro; iNext; iIntros (w) "#hthis".
+              rewrite (interp_tag_equivI _ _ _ heq A w).
+              by iApply "hcond".
+            }
+            iSplit; first done.
+            by rewrite (interp_tag_equivI _ _ _ heq A v).
         + iModIntro; iNext; iIntros (i c hc w) "#h1".
           assert (hc': subst_constraints σA (Δsdt A) !! i = Some (subst_constraint σA c)).
           { by rewrite /subst_constraints list_lookup_fmap hc. }
@@ -2116,8 +2877,15 @@ Section proofs.
             by eapply Δsdt_bounded in hc.
           }
           destruct hbc as [].
+          assert (hno: no_this_constraint c).
+          { destruct SDTCS.
+            by apply Δsdt_no_this in hc.
+          }
+          destruct hno as [].
+          rewrite (interp_type_no_this _ _ _ Σthis0 Σthis) //.
+          rewrite (interp_type_no_this _ _ _ Σthis0 Σthis) //.
           rewrite -!interp_type_subst //.
-          rewrite !interp_type_unfold.
+          rewrite !interp_type_unfold_v.
           iApply subtype_is_inclusion_aux => //.
           apply wf_ty_classI in hwfA.
           by apply wf_ty_subst.
@@ -2126,7 +2894,7 @@ Section proofs.
       - by iRight; iRight; iLeft.
       - done.
       - done.
-      - iDestruct ((subtype_is_inclusion_aux _ _ _ _ h (IntV 3)) with "wfΣ Σcoherency") as "hfalse".
+      - iDestruct ((subtype_is_inclusion_aux _ _ _ _ _ h (IntV 3)) with "wfThis wfΣ Σcoherency") as "hfalse".
         { by constructor. }
         iAssert (∃ z, ⌜IntV 3 = IntV z⌝)%I as "hh"; first by iExists _.
         rewrite /=.
@@ -2134,7 +2902,7 @@ Section proofs.
         by destruct hfalse.
     }
     move => hwfA hwfB.
-    destruct 1 as [ | ?????? h0 h1 h | ?????? h0 h | ?????? h0 h]; iIntros "#wfΣ #Σcoherency".
+    destruct 1 as [ | ?????? h0 h1 h | ?????? h0 h | ?????? h0 h]; iIntros "#wfThis #wfΣ #Σcoherency".
     - clear subtype_is_inclusion_aux subtype_targs_is_inclusion_aux.
       done.
     - simpl.
@@ -2166,27 +2934,29 @@ Section proofs.
   Qed.
 
   (* A <: B → [|A|] ⊆ [|B|] *)
-  Theorem subtype_is_inclusion kd Σ:
+  Theorem subtype_is_inclusion kd Σthis Σ:
     ∀ A B, subtype Δ kd A B →
     ∀ v,
     wf_ty A →
+    □ interp_as_mixed Σthis -∗
     □ interp_env_as_mixed Σ -∗
-    □ Σinterp Σ Δ -∗
-    interp_type A Σ v -∗ interp_type B Σ v.
+    □ Σinterp Σthis Σ Δ -∗
+    interp_type A Σthis Σ v -∗ interp_type B Σthis Σ v.
   Proof.
-    iIntros (A B hAB v ?) "#wfΣi #Σcoherency".
+    iIntros (A B hAB v ?) "#wfThis #wfΣ #Σcoherency".
     rewrite !interp_type_unfold.
-    by iApply (subtype_is_inclusion_aux with "wfΣi Σcoherency").
+    by iApply (subtype_is_inclusion_aux with "wfThis wfΣ Σcoherency").
   Qed.
 
-  Theorem inconsistency Σ kd:
+  Theorem inconsistency Σthis Σ kd:
     subtype Δ kd IntT BoolT →
+    □ interp_as_mixed Σthis -∗
     □ interp_env_as_mixed Σ -∗
-    □ Σinterp Σ Δ -∗
+    □ Σinterp Σthis Σ Δ -∗
     False%I.
   Proof.
-    iIntros (h) "#hmixed #hΣΔ".
-    iDestruct ((subtype_is_inclusion _ _ _ _ h (IntV 3)) with "hmixed hΣΔ") as "hfalse".
+    iIntros (h) "#hmixed0 #hmixed #hΣΔ".
+    iDestruct ((subtype_is_inclusion _ _ _ _ _ h (IntV 3)) with "hmixed0 hmixed hΣΔ") as "hfalse".
     { by constructor. }
     iAssert (∃ z, ⌜IntV 3 = IntV z⌝)%I as "hh"; first by iExists _.
     rewrite !interp_type_unfold /=.
@@ -2194,228 +2964,42 @@ Section proofs.
     by destruct hfalse.
   Qed.
 
-  Definition interp_this_def
-    (C: tag)
-    (Σ : list (interp Θ))
-    : interp Θ :=
-    Interp (
-      λ (w : value), (∃ ℓ t tdef σ (Σt: list (interp Θ))
-       (fields: stringmap ((visibility * lang_ty) * tag))
-       (ifields: gmapO string (sem_typeO Θ)),
-      ⌜w = LocV ℓ ∧
-       pdefs !! t = Some tdef ∧
-       length Σt = length tdef.(generics) ∧
-       inherits_using t C σ ∧
-       has_fields t fields ∧
-       dom fields = dom ifields⌝ ∗
-
-      □ ▷ interp_env_as_mixed Σt ∗
-
-      □ ▷ Σinterp Σt tdef.(constraints) ∗
-
-      ⌜((λ ty, interp_type ty Σt) <$> σ ≡ Σ)⌝ ∗
-
-      ▷ (∀ f vis ty orig, ⌜has_field f t vis ty orig⌝ -∗
-          (ifields !! f ≡ Some (interp_car (interp_type ty Σt)))) ∗
-
-      (ℓ ↦ (t, ifields)))%I
-    ).
-
-   Local Definition interp_this_aux
-     (C: tag)
-     (Σ : list (interp Θ))
-     : seal (@interp_this_def C Σ).
-   Proof. by eexists. Qed.
-
-   Definition interp_this C (Σ: list (interp Θ)) :=
-     (interp_this_aux C Σ).(unseal).
-
-   Definition interp_this_unseal C (Σ : list (interp Θ))
-     : interp_this C Σ = interp_this_def C Σ :=
-     (interp_this_aux C Σ).(seal_eq).
-
-  Definition interp_this_type C (σC: list lang_ty) Σ : interp Θ :=
-    interp_this C (interp_list Σ σC).
-
-  Lemma interp_this_type_app C σC: ∀ Σ0 Σ1,
-    bounded (length Σ0) (ClassT true C σC) →
-    interp_this_type C σC Σ0 ≡
-    interp_this_type C σC (Σ0 ++ Σ1).
-  Proof.
-    move => Σ0 Σ1 hb w.
-    rewrite /interp_this_type !interp_this_unseal /interp_this_def /interp_fun !interp_car_simpl.
-    do 18 f_equiv.
-    do 2 f_equiv.
-    rewrite /interp_list.
-    apply list_fmap_equiv_ext => ? ty hty.
-    apply elem_of_list_lookup_2 in hty.
-    apply interp_type_app.
-    apply boundedI in hb.
-    rewrite Forall_forall in hb.
-    by apply hb.
-  Qed.
-
-  Lemma interp_this_equivI (Σ0 Σ1: list (interp Θ)):
-    Σ0 ≡ Σ1 →
-    ∀ A v, interp_this A Σ0 v ≡ interp_this A Σ1 v.
-  Proof.
-    move => h A v.
-    rewrite !interp_this_unseal /interp_this_def /=.
-    by repeat f_equiv.
-  Qed.
-
-  Lemma this_extends_using_is_inclusion:
-    ∀ A B σ, extends_using A B σ →
-    ∀ Σ v,
-    interp_this A Σ v -∗
-    interp_this B (interp_list Σ σ) v.
-  Proof.
-    move => A B σ hext Σ v.
-    assert (hb: ∃ bdef, pdefs !! B = Some bdef ∧ length bdef.(generics) = length (interp_list Σ σ)).
-    { apply extends_using_wf in hext => //.
-      destruct hext as (? & ? & ? & h).
-      apply wf_tyI in h as (bdef & ? & ? & ?); simplify_eq.
-      exists bdef; repeat split => //.
-      by rewrite /interp_list fmap_length.
-    }
-    destruct hb as (bdef & hbdef & hlen2).
-    iIntros "h".
-    rewrite !interp_this_unseal /interp_this_def /=.
-    iDestruct "h" as (ℓ t tdef σin Σt fields ifields) "(%h & #hmixed & #hconstr & %hinst & hdyn & hl)".
-    destruct h as (-> & htdef & hlΣt & hin & hfields & hdom); simplify_eq.
-    destruct (extends_using_wf _ _ _ wf_parent hext) as (adef & hadef & hF & hwfB).
-    destruct (inherits_using_wf _ _ _ wf_parent hin) as (tdef' & htdef' & htF & hwfA).
-    simplify_eq.
-    iExists ℓ, t, tdef, (subst_ty σin <$> σ), Σt, fields, ifields.
-    iSplit.
-    { iPureIntro; repeat split => //.
-      by eapply inherits_using_trans; last by econstructor.
-    }
-    iSplitR => //.
-    iSplitR => //.
-    iSplitR; last by iSplit.
-    iPureIntro.
-    rewrite /interp_list -!list_fmap_compose.
-    apply list_fmap_equiv_ext => k ty hty v /=.
-    rewrite interp_type_subst; last first.
-    { replace (length σin) with (length adef.(generics)).
-      - rewrite Forall_lookup in hF.
-        by apply hF in hty.
-      - apply wf_tyI in hwfA as (? & ? & ? & ?); by simplify_eq.
-    }
-    by rewrite interp_type_equivI.
-  Qed.
-
-  Lemma this_inherits_using_is_inclusion:
-    ∀ Σ A B σA σB v, inherits_using A B σB →
-    wf_ty (ClassT true A σA) →
-    interp_this_type A σA Σ v -∗
-    interp_this_type B (subst_ty σA <$> σB) Σ v.
-  Proof.
-    move => Σ A B σA σB v h.
-    move : σA v.
-    induction h as [ A adef hpdefs | A B σ hext | A B σ C σC hext h hi ]
-        => σA v hwf.
-    - rewrite subst_ty_gen_targs; first done.
-      apply wf_tyI in hwf as (? & ? & ? & ?); by simplify_eq.
-    - iIntros "h".
-      destruct (extends_using_wf _ _ _ wf_parent hext) as (adef' & hadef' & hF & hwfB).
-      simplify_eq.
-      rewrite /interp_this_type.
-      iAssert (interp_this B (interp_list (interp_list Σ σA) σ) v)%I with "[h]" as "hh".
-      { by iApply this_extends_using_is_inclusion. }
-      rewrite interp_this_equivI; first done.
-      rewrite /interp_list -!list_fmap_compose.
-      apply list_fmap_equiv_ext => k ty hty w /=.
-      rewrite interp_type_subst; last first.
-      { replace (length σA) with (length adef'.(generics)).
-        - rewrite Forall_lookup in hF.
-          by apply hF in hty.
-        - apply wf_tyI in hwf as (? & ? & ? & ?); by simplify_eq.
-      }
-      by rewrite interp_type_equivI.
-    - iIntros "h".
-      iDestruct (this_extends_using_is_inclusion with "h") as "he" => //.
-      apply extends_using_wf in hext => //.
-      destruct hext as (? & ? & ? & hwfB).
-      rewrite map_subst_ty_subst; last first.
-      { apply inherits_using_wf in h => //.
-        destruct h as (bdef & hbdef & hb & hwfC).
-        replace (length σ) with (length bdef.(generics)); first done.
-        apply wf_tyI in hwfB as (? & ? & ? & ?); by simplify_eq.
-      }
-      iApply hi.
-      { assert (Forall wf_ty σA) by by apply wf_ty_classI in hwf.
-        assert (hσ: Forall wf_ty σ) by by apply wf_ty_classI in hwfB.
-        apply wf_tyI in hwfB as (? & ? & ? & ?).
-        apply wf_tyI in hwf as (? & ? & ? & ?).
-        simplify_eq.
-        econstructor => //.
-        - by rewrite map_length.
-        - rewrite Forall_lookup => k ? hty.
-          apply list_lookup_fmap_inv in hty as [ty [-> hty]].
-          apply wf_ty_subst => //.
-          rewrite Forall_lookup in hσ.
-          by apply hσ in hty.
-      }
-      rewrite interp_this_equivI; first done.
-      rewrite /interp_list -!list_fmap_compose.
-      apply list_fmap_equiv_ext => k ty hty w /=.
-      rewrite interp_type_subst; last first.
-      { replace (length σA) with (length x.(generics)).
-        - rewrite Forall_lookup in H0.
-          by apply H0 in hty.
-        - apply wf_tyI in hwf as (? & ? & ? & ?); by simplify_eq.
-      }
-      by rewrite interp_type_equivI.
-  Qed.
-
-  Definition interp_local_tys Σ
+  Definition interp_local_tys Σthis Σ
     (Γ : local_tys) (le : local_env) : iProp Θ :=
-    interp_this_type Γ.(type_of_this).1 Γ.(type_of_this).2 Σ (LocV le.(vthis)) ∗
-    (∀ v ty, ⌜Γ.(ctxt) !! v = Some ty⌝ -∗
-    ∃ val, ⌜le.(lenv) !! v = Some val⌝ ∗ interp_type ty Σ val)%I.
+    (Σthis (LocV le.(vthis))) ∗
+    (∀ v ty, ⌜Γ !! v = Some ty⌝ -∗
+     ∃ val, ⌜le.(lenv) !! v = Some val⌝ ∗ interp_type ty Σthis Σ val)%I.
 
-  Lemma interp_local_app Γ st Σ0 Σ1:
+  Lemma interp_local_app Γ st Σthis Σ0 Σ1:
     bounded_lty (length Σ0) Γ →
-    interp_local_tys Σ0 Γ st ≡
-    interp_local_tys (Σ0 ++ Σ1) Γ st.
+    interp_local_tys Σthis Σ0 Γ st ≡
+    interp_local_tys Σthis (Σ0 ++ Σ1) Γ st.
   Proof.
     move => hb.
     rewrite /interp_local_tys.
     f_equiv.
-    - rewrite -interp_this_type_app; first done.
-      destruct hb as [hb ?].
-      by eapply bounded_exact.
-    - iStartProof; iSplit; iIntros "h"; iIntros (v ty hv).
-      + iDestruct ("h" $! v ty hv) as (w hw) "#hw".
-        iExists w; iSplit; first done.
-        rewrite -interp_type_app; first done.
-        by apply hb in hv.
-      + iDestruct ("h" $! v ty hv) as (w hw) "#hw".
-        iExists w; iSplit; first done.
-        rewrite -interp_type_app; first done.
-        by apply hb in hv.
+    iStartProof; iSplit; iIntros "h"; iIntros (v ty hv).
+    + iDestruct ("h" $! v ty hv) as (w hw) "#hw".
+      iExists w; iSplit; first done.
+      rewrite -interp_type_app; first done.
+      by apply hb in hv.
+    + iDestruct ("h" $! v ty hv) as (w hw) "#hw".
+      iExists w; iSplit; first done.
+      rewrite -interp_type_app; first done.
+      by apply hb in hv.
   Qed.
 
-  Lemma interp_local_tys_is_inclusion kd Σ Γ0 Γ1 le:
+  Lemma interp_local_tys_is_inclusion kd Σthis Σ Γ0 Γ1 le:
     wf_lty Γ0 →
     Forall (λ (i: interp Θ), ∀ v, Persistent (i v)) Σ →
     lty_sub Δ kd Γ0 Γ1 →
+    □ interp_as_mixed Σthis -∗
     □ interp_env_as_mixed Σ -∗
-    □ Σinterp Σ Δ -∗
-    interp_local_tys Σ Γ0 le -∗
-    interp_local_tys Σ Γ1 le.
+    □ Σinterp Σthis Σ Δ -∗
+    interp_local_tys Σthis Σ Γ0 le -∗
+    interp_local_tys Σthis Σ Γ1 le.
   Proof.
-    move => hlty hpers hsub; iIntros "#wfΣ #? [#Hthis Hle]".
-    destruct hsub as [hthis hsub].
-    assert (hthis2: type_of_this Γ0 = type_of_this Γ1).
-    { rewrite /this_type in hthis.
-      rewrite (surjective_pairing (type_of_this Γ0))
-      (surjective_pairing (type_of_this Γ1)).
-      by case : hthis => -> ->.
-    }
-    rewrite /this_type hthis2.
+    move => hlty hpers hsub; iIntros "#wfThis #wfΣ #? [#Hthis Hle]".
     iSplitR; first done.
     iIntros (v ty) "%Hv".
     apply hsub in Hv as (B & hB & hsubB).
@@ -2595,21 +3179,23 @@ Section proofs.
     }
   Qed.
 
-  Lemma Δsdt_variance_interp: ∀ (Σ0 Σ1: list (interp Θ)) A adef,
+  Lemma Δsdt_variance_interp: ∀ Σthis (Σ0 Σ1: list (interp Θ)) A adef,
     map_Forall (λ _ : string, wf_cdef_mono) pdefs →
     map_Forall (λ _ : string, wf_cdef_parent pdefs) pdefs →
+    map_Forall (λ _cname, wf_cdef_constraints_no_this) pdefs →
     map_Forall (λ _cname, wf_cdef_constraints_bounded) pdefs →
     map_Forall (λ _cname, wf_cdef_constraints_wf) pdefs →
     pdefs !! A = Some adef →
+    □ interp_as_mixed Σthis -∗
     □ interp_env_as_mixed Σ0 -∗
     □ interp_env_as_mixed Σ1 -∗
     □ iForall3 interp_variance adef.(generics) Σ0 Σ1 -∗
-    □ Σinterp Σ0 adef.(constraints) -∗
-    □ Σinterp Σ1 adef.(constraints) -∗
-    □ Σinterp Σ1 (Δsdt A) -∗
-    □ Σinterp Σ0 (Δsdt A).
+    □ Σinterp Σthis Σ0 adef.(constraints) -∗
+    □ Σinterp Σthis Σ1 adef.(constraints) -∗
+    □ Σinterp Σthis Σ1 (Δsdt A) -∗
+    □ Σinterp Σthis Σ0 (Δsdt A).
   Proof.
-    move => Σ0 Σ1 A adef hwfp hwfm hwfbc hwfc hadef.
+    move => Σthis Σ0 Σ1 A adef hwfm hwfp hwfno hwfbc hwfc hadef.
     (* assume T0s and T1s such that for all i
      * T0i <:vi:> T1i
      *)
@@ -2630,9 +3216,9 @@ Section proofs.
               subst_constraints σ1 adef.(constraints) ++ subst_constraints σ1 (Δsdt A)).
     assert (hsub: Δentails Aware Δ (subst_constraints σ0 (Δsdt A))).
     { by eapply Δsdt_variance. }
-    iIntros "#hmixed0 #hmixed1 #hForall #hΣ0 #hΣ1 #h1".
+    iIntros "#hthism #hmixed0 #hmixed1 #hForall #hΣ0 #hΣ1 #h1".
     iDestruct (iForall3_length with "hForall") as "[%hlΣ0 %hlΣ1]".
-    iAssert (Σinterp (Σ0 ++ Σ1) Δ) with "[h1]" as "hΣΔ".
+    iAssert (Σinterp Σthis (Σ0 ++ Σ1) Δ) with "[h1]" as "hΣΔ".
     { rewrite /Δ.
       iApply Σinterp_app.
       { iIntros (i [U V] heq v) "#h"; simpl.
@@ -2644,13 +3230,13 @@ Section proofs.
         }
         case : w hw hUV => hw hUV.
         + case: hUV => [ [-> ->]| [-> ->]] /=.
-          * rewrite -(interp_type_app (GenT j) Σ0 Σ1) //.
+          * rewrite -(interp_type_app (GenT j) Σthis Σ0 Σ1) //.
             replace (GenT (j + n)) with (lift_ty (length Σ0) (GenT j)); last first.
             { by rewrite -hlΣ0. }
             rewrite interp_type_lift.
             iApply interp_with_mono => //.
             by constructor.
-          * rewrite -(interp_type_app (GenT j) Σ0 Σ1) //.
+          * rewrite -(interp_type_app (GenT j) Σthis Σ0 Σ1) //.
             replace (GenT (j + n)) with (lift_ty (length Σ0) (GenT j)); last first.
             { by rewrite -hlΣ0. }
             rewrite interp_type_lift.
@@ -2660,14 +3246,14 @@ Section proofs.
             constructor.
             by rewrite list_lookup_fmap hw.
         + case: hUV => -> -> /=.
-          rewrite -(interp_type_app (GenT j) Σ0 Σ1) //.
+          rewrite -(interp_type_app (GenT j) Σthis Σ0 Σ1) //.
           replace (GenT (j + n)) with (lift_ty (length Σ0) (GenT j)); last first.
           { by rewrite -hlΣ0. }
           rewrite interp_type_lift.
           iApply interp_with_mono => //.
           by constructor.
         + case: hUV => -> -> /=.
-          rewrite -(interp_type_app (GenT j) Σ0 Σ1) //.
+          rewrite -(interp_type_app (GenT j) Σthis Σ0 Σ1) //.
           replace (GenT (j + n)) with (lift_ty (length Σ0) (GenT j)); last first.
           { by rewrite -hlΣ0. }
           rewrite interp_type_lift.
@@ -2741,8 +3327,8 @@ Section proofs.
       apply hwfΔ in hck as [].
       split; simpl; by apply wf_ty_subst.
     }
-    iAssert (interp_type (subst_ty σ0 c.1) (Σ0 ++ Σ1) v -∗
-             interp_type (subst_ty σ0 c.2) (Σ0 ++ Σ1) v)%I as "hsub2".
+    iAssert (interp_type (subst_ty σ0 c.1) Σthis (Σ0 ++ Σ1) v -∗
+             interp_type (subst_ty σ0 c.2) Σthis (Σ0 ++ Σ1) v)%I as "hsub2".
     { iIntros "hh".
       assert (hwfcc: wf_constraint c).
       { rewrite Forall_lookup in hwfΔ.
@@ -2752,14 +3338,14 @@ Section proofs.
       { apply wf_ty_subst => //.
         by destruct hwfcc.
       }
-      by iApply (subtype_is_inclusion _ wfΣc hwfm hwfp hwfc hwfbc Aware (Σ0 ++ Σ1) _ _ hc0).
+      by iApply (subtype_is_inclusion _ wfΣc hwfp hwfm hwfc hwfno hwfbc Aware Σthis (Σ0 ++ Σ1) _ _ hc0).
     }
     assert (hbc: bounded_constraint (length (adef.(generics))) c).
     { by eapply Δsdt_bounded in hc. }
     destruct hbc as [].
     rewrite !subst_ty_id //.
-    rewrite (interp_type_app c.2 Σ0 Σ1); last by rewrite -hlΣ0.
-    rewrite (interp_type_app c.1 Σ0 Σ1); last by rewrite -hlΣ0.
+    rewrite (interp_type_app c.2 Σthis Σ0 Σ1); last by rewrite -hlΣ0.
+    rewrite (interp_type_app c.1 Σthis Σ0 Σ1); last by rewrite -hlΣ0.
     by iApply "hsub2".
   Qed.
 End proofs.
