theories/soundness/expr.v
@@ -14,47 +14,48 @@ From shack Require Import lang progdef subtype.
 From shack Require Import eval heap modality interp typing.
 
 Section proofs.
-  (* assume a given set of class definitions *)
-  Context `{PDC: ProgDefContext}.
-  (* assume some SDT constraints and their properties *)
-  Context `{SDTCS: SDTClassSpec}.
+  (* assume a given set of class definitions and their SDT annotations. *)
+  Context `{SDTCVS: SDTClassVarianceSpec}.
 
   (* Iris semantic context *)
   Context `{!sem_heapGS Θ}.
 
-  Lemma expr_soundness (Δ: list constraint) rigid (Σ: list (interp Θ)) kd e Γ Ω ty val :
+  Lemma expr_soundness (Δ: list constraint) rigid (Σthis: interp Θ)
+    (Σ: list (interp Θ)) kd e Γ Ω ty val :
     map_Forall (λ _, wf_cdef_parent pdefs) pdefs →
     map_Forall (λ _, wf_cdef_mono) pdefs →
     map_Forall (λ _ : string, wf_cdef_constraints_wf) pdefs →
+    map_Forall (λ _ : string, wf_cdef_constraints_no_this) pdefs →
     map_Forall (λ _ : string, wf_cdef_constraints_bounded) pdefs →
     Forall wf_constraint Δ →
     wf_lty Γ →
     expr_eval Ω e = Some val →
     expr_has_ty Δ Γ rigid kd e ty →
+    □ interp_as_mixed Σthis -∗
     □ interp_env_as_mixed Σ -∗
-    □ Σinterp Σ Δ -∗
-    interp_local_tys Σ Γ Ω -∗
-    interp_type ty Σ val.
+    □ Σinterp Σthis Σ Δ -∗
+    interp_local_tys Σthis Σ Γ Ω -∗
+    interp_type ty Σthis Σ val.
   Proof.
-    move => ????? wflty he h; move: Ω val he.
+    move => ?????? wflty he h; move: Ω val he.
     induction h as [| | | kd op e1 e2 hop he1 hi1 he2 hi2 |
         kd op e1 e2 hop he1 hi1 he2 hi2 | kd e1 e2 h1 hi1 h2 hi2 |
         kd e0 h hi | kd v vty hv | | kd exp S T hS hi hwf hok hsub |
         kd exp S T hS hi hwf hok hsub | kd e t hwf hb hsub ]
-        => Ω val he; iIntros "#wfΣ #Σcoherency #Hlty".
+        => Ω val he; iIntros "#wfThis #wfΣ #Σcoherency #Hlty".
     - case: he => <-; rewrite interp_type_unfold /=; by eauto.
     - case: he => <-; rewrite interp_type_unfold /=; by eauto.
     - case: he => <-; rewrite interp_type_unfold /=; by eauto.
     - simpl in he.
       case heq1 : (expr_eval Ω e1) => [v1 | ]; rewrite heq1 in he; last by done.
       apply hi1 in heq1.
-      iDestruct (heq1 with "wfΣ Σcoherency Hlty") as "hv1".
+      iDestruct (heq1 with "wfThis wfΣ Σcoherency Hlty") as "hv1".
       rewrite interp_type_unfold /=.
       iDestruct "hv1" as (z1) "%hz1".
       rewrite hz1 in he.
       case heq2 : (expr_eval Ω e2) => [v2 | ]; rewrite heq2 in he; last by done.
       apply hi2 in heq2.
-      iDestruct (heq2 with "wfΣ Σcoherency Hlty") as "hv2".
+      iDestruct (heq2 with "wfThis wfΣ Σcoherency Hlty") as "hv2".
       rewrite interp_type_unfold /=.
       iDestruct "hv2" as (z2) "%hz2".
       rewrite hz2 in he.
@@ -63,13 +64,13 @@ Section proofs.
     - simpl in he.
       case heq1 : (expr_eval Ω e1) => [v1 | ]; rewrite heq1 in he; last by done.
       apply hi1 in heq1.
-      iDestruct (heq1 with "wfΣ Σcoherency Hlty") as "hv1".
+      iDestruct (heq1 with "wfThis wfΣ Σcoherency Hlty") as "hv1".
       rewrite interp_type_unfold /=.
       iDestruct "hv1" as (z1) "%hz1".
       rewrite hz1 in he.
       case heq2 : (expr_eval Ω e2) => [v2 | ]; rewrite heq2 in he; last by done.
       apply hi2 in heq2.
-      iDestruct (heq2 with "wfΣ Σcoherency Hlty") as "hv2".
+      iDestruct (heq2 with "wfThis wfΣ Σcoherency Hlty") as "hv2".
       rewrite interp_type_unfold /=.
       iDestruct "hv2" as (z2) "%hz2".
       rewrite hz2 in he.
@@ -79,13 +80,13 @@ Section proofs.
     - simpl in he.
       case heq1 : (expr_eval Ω e1) => [v1 | ]; rewrite heq1 in he; last by done.
       apply hi1 in heq1.
-      iDestruct (heq1 with "wfΣ Σcoherency Hlty") as "hv1".
+      iDestruct (heq1 with "wfThis wfΣ Σcoherency Hlty") as "hv1".
       rewrite interp_type_unfold /=.
       iDestruct "hv1" as (b1) "%hb1".
       rewrite hb1 in he.
       case heq2 : (expr_eval Ω e2) => [v2 | ]; rewrite heq2 in he; last by done.
       apply hi2 in heq2.
-      iDestruct (heq2 with "wfΣ Σcoherency Hlty") as "hv2".
+      iDestruct (heq2 with "wfThis wfΣ Σcoherency Hlty") as "hv2".
       rewrite interp_type_unfold /=.
       iDestruct "hv2" as (b2) "%hb2".
       rewrite hb2 in he.
@@ -94,7 +95,7 @@ Section proofs.
     - simpl in he.
       case heq : (expr_eval Ω e0) => [v0 | ]; rewrite heq in he; last by done.
       apply hi in heq.
-      iDestruct (heq with "wfΣ Σcoherency Hlty") as "hv".
+      iDestruct (heq with "wfThis wfΣ Σcoherency Hlty") as "hv".
       rewrite interp_type_unfold /=.
       iDestruct "hv" as (b) "%hb".
       rewrite hb in he.
@@ -106,51 +107,7 @@ Section proofs.
       rewrite he in H; by case: H => ->.
     - case: he => <-.
       iDestruct "Hlty" as "[Hthis Hv]".
-      rewrite /interp_this_type interp_this_unseal /interp_this_def /=.
-      iDestruct "Hthis" as (?? tdef ????) "(%H & #hmixed & #hconstr & %hinst & hdyn & hloc)".
-      destruct H as ([= <-] & htdef & hl & hin & hfields & hdom).
-      rewrite /this_type interp_class_unfold //=; last first.
-      { eapply wf_ty_exact.
-        by apply wflty.
-      }
-      destruct Γ as [[this σthis] Γ]; simpl in *.
-      assert (hthis: wf_ty (ClassT true this σthis)).
-      { eapply wf_ty_exact.
-        by apply wflty.
-      }
-      apply wf_tyI in hthis as (thisdef & ? & hlen & ?).
-      iExists _,t,thisdef,tdef,_, _, _, _.
-      iSplit; first done.
-      iSplit; first by iApply "hmixed".
-      iSplit; first by iApply "hconstr".
-      iSplit; last by iSplit.
-      iModIntro; iNext.
-      iClear "wfΣ Σcoherency hmixed hdyn hloc Hv".
-      assert (hl0 : length thisdef.(generics) = length σ).
-      { apply inherits_using_wf in hin => //.
-        destruct hin as (?&?&?&h).
-        by inv h; simplify_eq.
-      }
-      assert (hl1: length σ = length σthis).
-      { by rewrite hlen. }
-      move : hl0 hl1 hinst.
-      generalize thisdef.(generics); clear.
-      move => l hl0 hl1 hinst.
-      iInduction l as [ | hd tl hi] "IH" forall (σ σthis hl0 hl1 hinst).
-      { by destruct σ; destruct σthis. }
-      destruct σ as [ | ty0 σ] => //=.
-      destruct σthis as [ | ty1 σthis] => //=.
-      case: hl0 => hl0.
-      case: hl1 => hl1.
-      rewrite /= cons_equiv_eq in hinst.
-      case : hinst => ? [? [h0 h1]].
-      case: h0 h1 => <- <- [h0 h1].
-      iSplitL.
-      + destruct hd; iIntros (w).
-        * iSplit; iIntros "h"; by rewrite h0.
-        * iIntros "h"; by rewrite h0.
-        * iIntros "h"; by rewrite h0.
-      + by iApply "IH".
+      by rewrite interp_type_unfold /=.
     - apply hi in he.
       iApply subtype_is_inclusion => //.
       + by apply expr_has_ty_wf in hS.
@@ -159,7 +116,7 @@ Section proofs.
       iApply subtype_is_inclusion => //.
       + by apply expr_has_ty_wf in hS.
       + by iApply he.
-    - by iDestruct (inconsistency with "wfΣ Σcoherency") as "hFalse".
+    - by iDestruct (inconsistency with "wfThis wfΣ Σcoherency") as "hFalse".
   Qed.
 End proofs.
 
